<section xml:id="section-bessel-functions">
  <title>Bessel Functions</title>
  <subsection xml:id="subsection-gamma-function">
    <title>The <m>\Gamma</m> Function</title>
    <p>
      Before we get to a very interesting example of the method of
      Frobenious, we need to define the <m>\Gamma</m> (gamma)function.
      This is a ubiquitous and useful function which generalizes the
      factorial.
    </p>
    <definition>
      <statement>
        <p>
          The <m>\Gamma</m> function is defined by this integral
          <me>
            \Gamma(t) = \int_0^\infty x^{t-1}e^{-x} dx
          </me>.
          The <m>\Gamma</m> function is defined on all <m>\RR</m>
          except 0 and negative integers. It is continuous and
          differentiable on <m>(0, \infty)</m>.
        </p>
      </statement>
    </definition>
    <p>
      There are several important properties of <m>\Gamma(t)</m>:
      First, (as mentioned) it generalizes the factorial.
      <md>
        <mrow>
          \Gamma(a+1) \amp = a \Gamma(a)
        </mrow>
        <mrow>
          \Gamma(1) \amp = 1
        </mrow>
        <mrow>
          \Gamma(n) \amp = (n-1)! \text{ for }  n \in \NN
        </mrow>
      </md>
    </p>
    <p>
      Asymptotically, the factorial nature of the <m>\Gamma</m>
      functions means it grows faster than <m>e^t</m>.
    </p>
    <p>
      If the positive integer values of the <m>\Gamma</m> function
      generalize the factorial, what can be expect for other values?
      The results are surprising. Look at the value of
      <m>\Gamma(\frac{1}{2})</m> (in this calculation, we use a
      well-known result for the integral <m>e^{-u^2}</m>).
      <md>
        <mrow>
          \Gamma \left( \frac{1}{2} \right) \amp = \int_0^\infty
          x^{-\frac{1}{2}} e^{-x} dx
        </mrow>
        <mrow>
          x \amp = u^2
        </mrow>
        <mrow>
          dx \amp = 2u du
        </mrow>
        <mrow>
          x^{-\frac{1}{2}} \amp = \frac{1}{u}
        </mrow>
        <mrow>
          \amp = 2 \int_0^\infty e^{-u^2} u \frac{1}{u} du
        </mrow>
        <mrow>
          \amp = 2 \int_0^\infty e^{-u^2}
        </mrow>
        <mrow>
          \amp = 2 \frac{\sqrt{\pi}}{2} = \sqrt{\pi}
        </mrow>
      </md>
    </p>
    <p>
      Then, from the factorial-like nature of <m>\Gamma</m>, all other
      half-integer values are multiples of <m>\sqrt{\pi}</m>.
      <me>
        \Gamma\left( \frac{2n+1}{2} \right) = \frac{ (3)(5)(7) \ldots
        (2n-1) \sqrt{\pi}}{2^n}
      </me>
    </p>
  </subsection>
  <subsection xml:id="subsection-bessel-equation">
    <title>Bessel's Equation</title>
    <p>
      The method of Frobenius is used to solve a historically
      interesting equation: Bessel's Equation. This equation shows up
      in harmonic problems with certain cirucular boundary conditions,
      such as the vibrations on a drum. It is also useful for springs
      with fatigue (where the spring constant gets weaker over time),
      the quantum model of the hydrogen atom, and various
      electical/gravitational potentials (particular those which are
      circularly or spherically symmetric). Its solutions are another
      piece of the mathematics of special functions.
    </p>
    <p>
      Let <m>\nu \in \RR</m>. Bessel's equation of order <m>\nu</m>
      is the equation
      <me>
        t^2 y^{\prime \prime} + t y^\prime + (t^2 - \nu^2) y = 0
      </me>.
      Written in standard form, <m>0</m> is a regular singular point
      of Bessel's equation.
      <md>
        <mrow>
          P(t) \amp = \frac{1}{t} \implies p_{-1} = 1
        </mrow>
        <mrow>
          Q(t) \amp = 1-\frac{\nu^2}{t^2} \implies q_{-2} = -\nu^2
        </mrow>
      </md>
    </p>
    <p>
      We calculate the indicial equation.
      <md>
        <mrow>
          r(r-1) + r - \nu^2 \amp = 0
        </mrow>
        <mrow>
          r^2 -r + r - \nu^2 \amp = 0
        </mrow>
        <mrow>
          r^2 \amp = \nu^2
        </mrow>
        <mrow>
          r \amp = \pm \nu
        </mrow>
      </md>
    </p>
    <p>
      We start with <m>r = \nu</m> first and assume that <m>\nu \geq
      0</m> without loss of generality. We calculate the derivatives
      of <m>y</m>.
      <md>
        <mrow>
          y \amp = \sum_{n=0}^\infty c_n t^{n+\nu}
        </mrow>
        <mrow>
          y^\prime \amp = \sum_{n=0}^\infty c_n(n+\nu) t^{n+\nu- 1}
        </mrow>
        <mrow>
          y^{\prime\prime} \amp = \sum_{n=0}^\infty
          c_n(n+\nu)(n+\nu-1) t^{n+\nu- 2}
        </mrow>
      </md>
    </p>
    <p>
      Then we proceed with a lengthly calculation.
      <md>
        <mrow>
          t^2 y^{\prime \prime} + t y^\prime + (t^2 - \nu^2) y \amp =
          0
        </mrow>
        <mrow>
          t^2 \sum_{n=0}^\infty c_n(n+\nu)(n+\nu-1) + t
          \sum_{n=0}^\infty c_n(n+\nu) t^{n+\nu- 1} + t^2
          \sum_{n=0}^\infty c_n t^{n+\nu} - \nu^2 \sum_{n=0}^\infty
          c_n t^{n+\nu} \amp = 0
        </mrow>
        <mrow>
          \sum_{n=0}^\infty c_n(n+\nu)(n+\nu-1) t^{n+\nu} +
          \sum_{n=0}^\infty c_n(n+\nu) t^{n+\nu} + \sum_{n=0}^\infty
          c_n t^{n+\nu+2} - \sum_{n=0}^\infty \nu^2 c_n t^{n+\nu} \amp
          = 0
        </mrow>
        <mrow>
          \sum_{n=0}^\infty c_n(n+\nu)(n+\nu-1) t^{n+\nu} +
          \sum_{n=0}^\infty c_n(n+\nu) t^{n+\nu} + \sum_{n=2}^\infty
          c_{n-2} t^{n+\nu} - \sum_{n=0}^\infty \nu^2 c_n t^{n+\nu}
          \amp = 0
        </mrow>
        <mrow>
          \nu(\nu-1) c_0 t^\nu + (\nu+1) \nu c_1 t^{\nu+1} + \nu c_0
          t^\nu + (\nu+1)c_1t^{\nu+1} - \nu^2 c_0 t^\nu - \nu^2 c_1
          t^{\nu+1} \amp
        </mrow>
        <mrow>
          + \sum_{n=2}^\infty c_n(n+\nu)(n+\nu-1) t^{n+\nu} +
          \sum_{n=2}^\infty c_n(n+\nu) t^{n+\nu} + \sum_{n=2}^\infty
          c_{n-2} t^{n+\nu} - \sum_{n=2}^\infty \nu^2 c_n t^{n+\nu}
          \amp = 0
        </mrow>
        <mrow>
          \nu(\nu-1) c_0 t^\nu + (\nu+1) \nu c_1 t^{\nu+1} + \nu c_0
          t^\nu + (\nu+1)c_1t^{\nu+1} - \nu^2 c_0 t^\nu - \nu^2 c_1
          t^{\nu+1} \amp
        </mrow>
        <mrow>
          + \sum_{n=2}^\infty \left[ c_n(n+\nu)(n+\nu-1) + c_n(n+\nu)
          + c_{n-2} - \nu^2 c_n \right] t^{n+\nu} \amp = 0
        </mrow>
      </md>
    </p>
    <p>
      Look at the coefficient of <m>t^{\nu}</m>.
      <md>
        <mrow>
          \left( (\nu^2 - \nu) c_0 +\nu c_0 - \nu^2 c_0 \right) \amp =
          0
        </mrow>
        <mrow>
          \left( \nu^2 - \nu + \nu - \nu^2 \right) c_0 \amp = 0
        </mrow>
        <mrow>
          0 c_0 \amp = 0
        </mrow>
      </md>
    </p>
    <p>
      Therefore, <m>c_0</m> is free. Look at the coefficient of
      <m>t^{\nu+1}</m>.
      <md>
        <mrow>
          \left( \nu(\nu+1)c_1 + (\nu+1) c_1 - \nu^2 c_1 \right) \amp
          = 0
        </mrow>
        <mrow>
          \left( \nu^2 + \nu + \nu + 1 - \nu^2 \right) c_1 \amp = 0
        </mrow>
        <mrow>
          \left( 2 \nu + 1 \right) c_1 \amp =0
        </mrow>
      </md>
    </p>
    <p>
      So <m>c_1 = 0</m> unless <m>\nu = \frac{-1}{2}</m>. However, we
      assumed that we were dealing with <m>\nu</m> positive, so we
      conclude that <m>c_1 = 0</m>. (We'll pay some special attention
      to <m>\nu = \frac{-1}{2}</m> when we look at negative
      <m>\nu</m>, and to half-integer values of <m>\nu</m> in
      general.)
    </p>
    <p>
      Then we have the general recurrence relation, for <m>n \geq
      2</m>.
      <md>
        <mrow>
          ((n+\nu)(n+\nu-1) + n + \nu - \nu^2) c_n + c_{n-2} \amp = 0
        </mrow>
        <mrow>
          (n^2 + n\nu + n\nu + \nu^2 - n - \nu + n + \nu - \nu^2 ) c_n
          \amp = -c_{n-2}
        </mrow>
        <mrow
          >
          (n^2 + 2n\nu) c_n \amp = -c_{n-2}
        </mrow>
        <mrow>
          c_n \amp = \frac{-c_{n-2}}{n(n+2\nu)}
        </mrow>
        <mrow>
          c_{n+2} \amp = \frac{-c_n}{(n+2)(n+2+2\nu)}
        </mrow>
      </md>
    </p>
    <p>
      These are the equations that calculate coefficients, so we start
      calculating.
      <md>
        <mrow>
          c_0 \amp = c_0
        </mrow>
        <mrow>
          (2\nu+1) c_1 \amp = 0 \implies c_1 = 0 \implies c_{2n+1} = 0
          \ \forall n \in \NN
        </mrow>
        <mrow>
          c_2 \amp = \frac{-c_0}{2(2+2\nu)}
        </mrow>
        <mrow>
          c_4 \amp = \frac{c_0}{(2)(4)(2+2\nu)(4+2\nu)}
        </mrow>
        <mrow>
          c_6 \amp = \frac{-c_0}{(2)(4)(6)(2+2\nu)(4+2\nu)(6+2\nu)}
        </mrow>
        <mrow>
          c_8 \amp = \frac{c_0}{(2)(4)(6)(8)(2+2\nu)(4+2\nu)(6+2\nu)
          (8+2\nu)}
        </mrow>
        <mrow>
          c_{2n} \amp = \frac{(-1)^n c_0}{2^{2n} n! (1+\nu)(2+\nu)
          \ldots (n+\nu)}
        </mrow>
      </md>
    </p>
    <p>
      The constant <m>c_0</m> is still undetermined. By convention,
      the choice for <m>c_0</m> is this strange value
      <me>
        c_0 = \frac{1}{2^\nu \Gamma(1+\nu)}
      </me>.
      The properties of the <m>\Gamma</m> function allow us to
      simplify the denominator of the <m>c_n</m>.
      <me>
        c_{2n} = \frac{(-1)^n}{2^\nu \Gamma(1+\nu)} \frac{1}{2^{2n}n!
        (\nu+1) \ldots (\nu+n)} = \frac{(-1)^n}{2^{2n+v} n!
        \Gamma(1+n+\nu)}
      </me>
      With this simplification, we can write the final solution for
      positive <m>\nu</m>.
    </p>
    <definition>
      <statement>
        <p>
          The solution constructed above is written <m>J_\nu</m> and
          called the Bessel function of the first kind of order
          <m>\nu</m>.
          <me>
            J_{\nu} = \sum_{n=0}^\infty \frac{(-1)^n}{n!
            \Gamma(1+n+\nu)} \left( \frac{t}{2} \right)^{2n+\nu}
          </me>
          It converges on <m>(0, \infty)</m>. It may not be defined
          at 0 or negative numbers. In general, we are only
          interested in the Bessel function on the domain <m>(0,
          \infty)</m>. The Bessel functions of the first kind for
          <m>\nu \in \ZZ</m> are show in <xref
          ref="figure-bessel-first-kind" />.
        </p>
      </statement>
    </definition>
    <figure xml:id="figure-bessel-first-kind">
      <caption>Integer-Order Bessel Functions of the First Kind</caption>
      <image xml:id="figure21" width="80%">
        <asymptote>
          size(8cm,6cm,IgnoreAspect); 
          import graph;
          import gsl; 
          
          xaxis(Ticks());
          yaxis(Ticks());
          
          typedef real realfcn(real); 
          realfcn F(int p) { 
            return new real(real x) {return Jn(p,x);}; 
          }; 
           
          for(int i=1; i \lt 7; ++i)
            draw(graph(F(i),0,12),Pen(i));
        </asymptote>
      </image>
    </figure>
    <figure xml:id="figure-bessel-second-kind">
      <caption>Integer-Order Bessel Functions of the Second Kind</caption>
      <image xml:id="figure22" width="80%">
        <asymptote>
          size(8cm,6cm,IgnoreAspect); 
          import graph;
          import gsl; 

          xaxis(Ticks());
          yaxis(Ticks());

          typedef real realfcn(real); 
          realfcn F(int p) { 
            return new real(real x) {return Yn(p,x);}; 
          }; 
 
          draw(graph(F(1),1,16),Pen(1));
          draw(graph(F(2),2,16),Pen(2));
          draw(graph(F(3),3,16),Pen(3));
          draw(graph(F(4),4,16),Pen(4));
          draw(graph(F(5),5,16),Pen(5));
          draw(graph(F(6),6,16),Pen(6));
        </asymptote>
      </image>
    </figure>
    <p>
      We could redo the same work for negative <m>\nu</m>, but it is
      very similar (for <m>n = \frac{-1}{2}</m>, we would get a term
      <m>(2\nu - 1) c_1</m>, so we would still conclude that <m>c_1 =
      0</m>, hence all odd coefficients are <m>0</m>). In this way,
      we find the rest of the Bessel functions of the first kind.
      <me>
        J_{-\nu} = \sum_{n=0}^\infty \frac{(-1)^n}{n! \Gamma(1+n-\nu)}
        \left( \frac{t}{2} \right)^{2n-\nu}
      </me>
      One caution should be noted. If <m>n \in \NN</m>, this
      <m>J_{-n}</m> gives an undefined denominator, hence doesn't
      define a series. In these cases, the method of Frobenius gives
      <m>J_{-n} = (-1)^n J_{n}</m>. This is not necessarily
      surprising: in the method of Frobenius, is the roots of the
      indicial equation differ by an integer, we may not have linearly
      independent solution. If <m>\nu \notin \ZZ</m>, then we have
      two linearly independent solutions, as we would expect with the
      method of Frobenius.
    </p>
    <definition>
      <statement>
        <p>
          Let <m>n \notin \ZZ</m>. The <term>Bessel function of the
          second kind</term> of order <m>\nu</m> are written
          <m>Y_{\nu}</m> and defined by this expression
          <me>
            Y_{\nu} = \frac{\cos (\nu \pi) J_{\nu}(t) -
            J_{-\nu}(t)}{\sin \nu \pi}
          </me>.
          This definition is a linear combination of Bessel functions
          of the first kind. For <m>\nu \in \ZZ</m>, this linear
          combination have been just a multiple of the one solution we
          know. To get around this, for <m>\nu \in \ZZ</m>, we define
          the Bessel function of the second kind as a limit.
          <me>
            Y_{\nu}(t) = \lim_{\alpha \rightarrow \nu} Y_{\alpha}(t)
          </me>
          L'Hopital's rule shows that this limit exists. The Bessel
          functions of the second kind are shown in <xref
          ref="figure-bessel-second-kind" />.
        </p>
      </statement>
    </definition>
    <p>
      To summarize, for any <m>\nu \geq 0</m> we have <m>J_{\nu}</m>
      and <m>Y_{\nu}</m>, two linearly independent solutions to the
      differential equation. The general solution is
      <me>
        y = A J_{\nu} + B Y_{\nu}
      </me>.
    </p>
  </subsection>
  <subsection xml:id="subsection-aging-spring">
    <title>The Aging Spring</title>
    <p>
      Consider the spring equation from before.
      <me>
        my^{\prime \prime} + by^\prime + ky = 0
      </me>
      Now, instead of all constants, lets assume this is an aging
      spring. That is, at time passes, the spring constant decreases.
      One model is exponential decay, so let <m>k(t) = ke^{-\alpha
      t}</m> for <m>\alpha > 0</m>. Let's see what happens without
      friction.
      <me>
        m y^{\prime \prime} + ke^{-\alpha t} = 0
      </me>
      Here's a strange change of variables.
      <md>
        <mrow>
          s \amp = \frac{2}{\alpha} \sqrt{\frac{k}{m}}
          e^{\frac{-\alpha t}{2}}
        </mrow>
        <mrow>
          \frac{ds}{dt} \amp = \frac{2}{\alpha} \frac{-\alpha}{2}
          \sqrt{ \frac{4k}{m\alpha^2}} e^{\frac{-\alpha t}{2}} = -
          \sqrt{\frac{k}{m}} e^{-\frac{\alpha t}{2}}
        </mrow>
        <mrow>
          \frac{d^2s}{dt^2} \amp = \frac{\alpha}{2} \sqrt{\frac{k}{m}}
          e^{-\frac{\alpha t}{2}}
        </mrow>
        <mrow>
          \frac{dy}{dt} \amp = \frac{dy}{ds} \frac{ds}{dt}
        </mrow>
        <mrow>
          \frac{d^2 y}{dt^2} \amp = \frac{d}{dt} \left( \frac{dy}{ds}
          \frac{ds}{dt} \right)
        </mrow>
        <mrow>
          \amp = \frac{d^2 s}{dt^2} \frac{dy}{ds} + \frac{ds}{dt}
          \frac{d}{dt} \frac{dy}{ds}
        </mrow>
        <mrow>
          \amp = \frac{d^2 s}{dt^2} \frac{dy}{ds} + \frac{ds}{dt}
          \frac{d^2y}{ds^2} \frac{ds}{dt}
        </mrow>
        <mrow>
          \amp = \frac{d^2 s}{dt^2} \frac{dy}{ds} + \left(
          \frac{ds}{dt} \right)^2 \frac{d^2 y}{ds^2}
        </mrow>
        <mrow>
          \amp = \frac{\alpha}{2} \sqrt{\frac{k}{m}} e^{-\frac{\alpha
          t}{2}} \frac{dy}{ds} + \frac{k}{m} e^{-\alpha t} \frac{d^2
          y}{ds^2}
        </mrow>
      </md>
    </p>
    <p>
      All this nonsense allows us to alter the original equation as
      follows. (The change from the third to the fourth line involves
      dividing by <m>m</m>, then dividing by <m>\alpha^2</m>, then
      multiplying by 4.)
      <md>
        <mrow>
          m y^{\prime \prime} + ke^{-\alpha t} \amp = 0
        </mrow>
        <mrow>
          m \left(\frac{d^2 s}{dt^2} \frac{dy}{ds} + \left(
          \frac{ds}{dt} \right)^2 \frac{d^2 y}{ds^2} \right) +
          ke^{-\alpha t} \amp = 0
        </mrow>
        <mrow>
          \frac{m\alpha}{2} \sqrt{\frac{k}{m}} e^{-\frac{\alpha t}{2}}
          \frac{dy}{ds} + m \frac{k}{m} e^{-\alpha t} + k e^{-\alpha
          t} y \amp = 0
        </mrow>
        <mrow>
          \frac{2}{\alpha} \sqrt{\frac{k}{m}} e^{-\frac{\alpha t}{2}}
          \frac{dy}{ds} + \frac{4}{\alpha^2} \frac{k}{m} e^{-\alpha t}
          \frac{d^y}{ds^2} + \frac{4k}{m\alpha^2} e^{-\alpha t} y \amp
          = 0
        </mrow>
        <mrow>
          s^2 \frac{d^2y}{ds^2} + s \frac{dy}{ds} + s^2 y \amp = 0
        </mrow>
      </md>
    </p>
    <p>
      This is Bessel's equation with <m>\nu = 0</m>. It is solved by
      Bessel's functions (of the first and second kind) for <m>\nu =
      0</m>.
      <md>
        <mrow>
          y \amp = A J_0(s) + B Y_0(s)
        </mrow>
        <mrow>
          \amp = A J_0 \left( \frac{2}{\alpha} \sqrt{\frac{k}{m}}
          e^{-\frac{\alpha t}{2}} \right) + B Y_0 \left(
          \frac{2}{\alpha} \sqrt{\frac{k}{m}} e^{-\frac{\alpha t}{2}}
          \right)
        </mrow>
      </md>
    </p>
    <p>
      These functions completely describe the behaviour of an aging
      spring with exponential decay of the spring constant.
    </p>
  </subsection>
  <subsection xml:id="subsection-bessel-functions-properties">
    <title>Properties of the Bessel Functions</title>
    <p>
      We have some nice symmetry properties for integer orders. Let
      <m>m \in \ZZ</m>.
      <md>
        <mrow>
          J_{-m}(t) \amp = (-1)^m J_m(t)
        </mrow>
        <mrow>
          J_m(-t) \amp = (-1)^m J_m(t)
        </mrow>
      </md>
    </p>
    <p>
      We mentioned a functional equation for the Legendre polynomials.
      We have one here as well; this one is true for arbitrary
      <m>\nu</m>.
      <me>
        tJ_{\nu}^\prime(t) = \nu J_{\nu}(t) - t J_{\nu+1}(t)
      </me>
      There are some interesting properties of Bessel functions with
      half-integer orders. Look closely again at
      <m>J_{\frac{1}{2}}</m>.
      <md>
        <mrow>
          J_{\frac{1}{2}}(t) \amp = \sum_{n=0}^\infty \frac{(-1)^n}{n!
          \Gamma(\frac{3}{2} + n))} \left( \frac{t}{2} \right)^{2n +
          \frac{1}{2}}
        </mrow>
        <mrow>
          \Gamma \left( \frac{3}{2} + n \right) \amp =
          \frac{(2n+1)!}{2^{2n+1} n!} \sqrt{\pi}
        </mrow>
        <mrow>
          J_{\frac{1}{2}}(t) \amp = \sum_{n=0}^\infty \frac{(-1)^n}
          {\frac{(2n+1)!}{2^{2n+1}n!} \sqrt{\pi}} \left( \frac{t}{2}
          \right)^{2n + \frac{1}{2}}
        </mrow>
        <mrow>
          \amp = \sqrt{\frac{2}{\pi t}} \sum_{n=0}^\infty
          \frac{(-1)^n}{(2n+1)!} t^{2n+1}
        </mrow>
        <mrow>
          \amp = \sqrt{\frac{2}{\pi t}} \sin t
        </mrow>
        <mrow>
          J_{-\frac{1}{2}} \amp = \sqrt{\frac{2}{\pi t}} \cos t
        </mrow>
      </md>
    </p>
    <p>
      These special half-integer function can actually be expressed as
      elementary functions. The decay of the amplitude of these waves
      is <m>\frac{1}{\sqrt{t}}</m> not <m>e^{-t}</m>; this decay is
      much slower than exponential decay. The half-integer Bessel
      functions are called <em>spherical Bessel functions</em>. The
      reason for that name is that they solve the wave equation in
      spherical coordinates. The wave equation in <m>\RR^3</m> is
      <m>\nabla^2 A + k^2 A = 0</m> for <m>\nabla^2</m> the Laplacian.
      Changing to spherical coordinates and restricting to the radial
      terms gives Bessel's equation with half-integer order.
    </p>
    <p>
      We can think of these half-integer Bessel functions as the
      standing waves of spherical harmonic systems.
      <m>J_{\frac{1}{2}}</m> is the first harmoinc, then we get higher
      harmonics as we go. The typical image of these spherical waves
      are the decaying amplitude ripples radiating from a stone
      dropped in a pond.
    </p>
  </subsection>
</section>
