<section xml:id="laplace-examples">
  <title>More Examples of Solving DEs with Laplace
  Transforms</title>
  <example>
    <statement>
      <p>
        Consider a slightly different version of the square wave.
        <me>
          f(t) = \left\{ \begin{matrix} 1 \amp  t \in [2n, 2n+1) \\ -1 \amp  t \in [2n+1, 2n+2) \end{matrix} \right.
        </me>
      </p>
      <p>
        Using initial conditions <m>y(0) = y^\prime(0)= 0</m> we solve the equation <m>y^{\prime \prime} + y = f(t)</m>.
        <md>
          <mrow>(s^2+1)Y \amp  = \frac{1}{1-e^{-2s}} \int_0^2 e^{-st} f(t) dt</mrow>
          <mrow>\amp  = \frac{1}{1-e^{-2s}} \left[ \int_0^1 e^{-st} dt - \int_1^2 e^{-st} dt \right]</mrow>
          <mrow>\amp  = \frac{1}{1-e^{-2s}} \left[ \left. \frac{e^{-st}}{-s} \right|_0^1 + \left. \frac{e^{-st}}{s} \right|_1^2 \right]</mrow>
          <mrow>\amp  = \frac{1}{1-e^{2s}} \left[ \frac{-e^{-s}}{s} + \frac{1}{s} + \frac{e^{-2s}}{s} - \frac{e^{-s}}{s} \right]</mrow>
          <mrow>\amp  = \frac{1-2s^{-s} + e^{-2s}}{s(s^2+1)} \frac{1}{1-e^{-2s}}</mrow>
          <mrow>\amp  = \frac{1}{s(s^2+1)} (1-2e^{-s} + e^{-2s}) ( 1 - e^{-2s} + e^{-4s} - e^{-6s} + e^{-8s} - \ldots )</mrow>
          <mrow>\amp  = \left( \frac{-s}{s+1} + \frac{1}{s} \right) (1 - 2e^{-s} + 2e^{-3s} - 2e^{-5s} + 2e^{-7s} - \ldots )</mrow>
          <mrow>y \amp  = 1 - \cos t - 2u_1(t) (1-\cos(t-1)) + 2u_3(t) (1-\cos(t-3))</mrow>
          <mrow>\amp  \hspace{1cm} - 2u_5 (t) (1-\cos(t-5)) + 2 u_7(t) (1 - \cos (t-7) ) - \ldots</mrow>
          <mrow>\amp  = 1 - \cos t + 2\sum_{k=0}^\infty (-1)^{k+1} u_{2k+1} (t) (1 - \cos(t-(2k+1)))</mrow>
        </md>
      </p>
      <p>
        As with the previous square wave solution in <xref ref="example-square-wave">Example</xref>,
        this solution involves an infinite series of shifts,
        each one slightly further along.
        Periodic functions always lead to an infinite series of shifts.
      </p>
    </statement>
  </example>
  <example>
    <statement>
      <p>
        This examples also involves a step function.
        <md>
          <mrow>y^{\prime \prime} + 6y^\prime + 5y \amp  = t - tu_2(t) \hspace{1cm} y(0) = 1 \hspace{1cm} y^\prime(0) = 0</mrow>
          <mrow>s^2 Y - s + 6sY - 6 + 5Y \amp  = \frac{1}{s^2} - e^{-2s} \left( \frac{1}{s^2} - \frac{2}{s} \right)</mrow>
          <mrow>(s+5)(s+1) Y \amp  = \frac{1}{s^2} - \frac{e^{-2s}}{s^2} + \frac{2e^{-2s}}{s} + s + 6</mrow>
          <mrow>Y \amp  = \frac{1}{s^2(s+1)(s+5)} - \frac{e^{-2s}}{s^2(s+1)(s+5)} + \frac{2e^{-2s}}{s(s+1)(s+5)}</mrow>
          <mrow>\amp  \hspace{1cm} + \frac{s}{(s+5)(s+1)} + \frac{6}{(s+5)(s+1)}</mrow>
          <mrow>\amp  = \frac{1}{5s^2} + \frac{1}{4(s+1)} - \frac{1}{100(s+5)} - \frac{6}{25s} - \frac{e^{-2s}}{5s^2} - \frac{e^{-2s}}{4(s+1)} + \frac{e^{-2s}}{100(s+5)}</mrow>
          <mrow>\amp  \hspace{1cm} + \frac{6e^{-2s}}{25s} - \frac{e^{-2s}}{2(s+1)} + \frac{e^{-2s}}{10(s+5)} + \frac{2e^{-2s}}{5s} + \frac{5}{4(s+5)} - \frac{1}{4(s+1)}</mrow>
          <mrow>\amp  \hspace{1cm} - \frac{3}{2(s+1)} + \frac{3}{2(s+5)}</mrow>
          <mrow>Y \amp  = \frac{1}{5s^2} - \frac{6}{25s} + \frac{3}{20(s+1)} + \left( \frac{-1}{100} + \frac{5}{4} + \frac{3}{2} \right) \frac{1}{s+5}</mrow>
          <mrow>\amp  \hspace{1cm} + e^{-2s} \left( \frac{1}{5s^2} + \left( \frac{6}{25} + \frac{2}{5} \right) \frac{1}{s} + \left( \frac{-1}{4} - \frac{1}{2} \right) \frac{1}{s+1} + \left(\frac{1}{100} + \frac{1}{10} \right) \frac{1}{s+5} \right)</mrow>
          <mrow>\amp  = \frac{1}{5s^2} - \frac{6}{25s} - \frac{3}{2(s+1)} + \frac{137}{50(s+5)}</mrow>
          <mrow>\amp  \hspace{1cm} + e^{-2s} \left( \frac{1}{5s^2} + \frac{16}{25s} - \frac{3}{4(s+1)} + \frac{11}{100(s+5)} \right)</mrow>
          <mrow>y \amp  = \frac{t}{5} - \frac{6}{25} - \frac{3e^{-t}}{2} + \frac{137e^{-5t}}{50} + u_2(t) \left[ \frac{(t-2)}{5} + \frac{16}{25} - \frac{3e^{2-t}}{4} + \frac{11e^{10-5t}}{100} \right]</mrow>
          <mrow>y \amp  = \frac{t}{5} - \frac{6}{25} - \frac{3e^{-t}}{2} + \frac{137e^{-5t}}{50} + u_2(t) \left[ \frac{t}{5} + \frac{6}{25} - \frac{3e^{2-t}}{4} + \frac{11e^{10-5t}}{100} \right]</mrow>
        </md>
      </p>
    </statement>
  </example>
  <example>
    <statement>
      <p>
        This example uses two <m>\delta</m>-functions,
        representing two sudden impacts.
        <md>
          <mrow>y^{\prime \prime} - 7y^\prime + 6y \amp  = e^t + \delta_2(t) + \delta_4(t) \hspace{1cm} y(0) = y^\prime(0) = 0</mrow>
          <mrow>s^2 Y - 7sY + 6Y \amp  = \frac{1}{s-1} + e^{-2s} + e^{-4s}</mrow>
          <mrow>Y \amp  = \frac{1}{(s-1)(s-6)(s-1)} + \frac{e^{-2s}}{(s-6)(s-1)} + \frac{e^{-4s}}{(s-6)(s-1)}</mrow>
          <mrow>\amp  = \frac{-1}{25(s-1)} - \frac{1}{5(s-1)^2} + \frac{1}{25(s-6)}</mrow>
          <mrow>\amp  \hspace{1cm} + e^{-2t} \left( \frac{1}{5(s-6)} - \frac{1}{5(s-1)} \right)</mrow>
          <mrow>\amp  \hspace{1cm} + e^{-4t} \left( \frac{1}{5(s-6)} - \frac{1}{5(s-1)} \right)</mrow>
          <mrow>y \amp  = \frac{e^{-t}}{25} - \frac{1}{2} \calL^{-1} \left\{ \frac{d}{dt} \frac{-1}{s-1} \right\} + \frac{1}{25} e^{6t}</mrow>
          <mrow>\amp  \hspace{1cm} \frac{u_2(t)}{5} \left( e^{6(t-2)}- e^{t-2} \right) + \frac{u_4(t)}{5} \left( e^{6(t-4)}- e^{t-4} \right)</mrow>
          <mrow>y \amp  = \frac{e^{-t}}{25} - \frac{te^t}{5} + \frac{1}{25} e^{6t}</mrow>
          <mrow>\amp  \hspace{1cm} \frac{u_2(t)}{5} \left( e^{6t-12}- e^{t-2} \right) + \frac{u_4(t)}{5} \left( e^{6t-24}- e^{t-4} \right)</mrow>
        </md>
      </p>
    </statement>
  </example>
  <example>
    <statement>
      <p>
        This is a ridiculous example with infinitely many <m>\delta</m>-functions,
        representing a new impact at every unit of time.
        <md>
          <mrow>f(t) \amp  = \sum_{n=0}^\infty \delta_n (t)</mrow>
          <mrow>y^{\prime \prime} + 3 y^\prime + 2y \amp  = f(t) \hspace{1cm} y(0) = y^\prime(0) = 0</mrow>
          <mrow>s^2 Y + 3sY + 2Y \amp  = \frac{1}{1-e^{-s}} \int_0^1 e{-st} \delta_0 (t) dt = \frac{1}{1-e^{-s}}</mrow>
          <mrow>Y \amp  = \frac{1}{1-e^{-s}} \frac{1}{(s+2)(s+1)}</mrow>
          <mrow>Y \amp  = \left( \frac{1}{s+1} - \frac{1}{s+2} \right) \left( 1 _ e^{-s} + e^{-2s} + e^{-3s} + e^{-4s} + \ldots \right)</mrow>
          <mrow>y \amp  = e^{-t} - e^{-2t} + u_1(t) \left( e^{-(t-1)} - e^{-(2t-2)} \right) + u_2(t) \left( e^{-(t-2)} - e^{-(2t-4)} \right)</mrow>
          <mrow>\amp  \hspace{1cm} + u_3(t) \left( e^{-(t-3)} - e^{-(2t-6)} \right) + u_4(t) \left( e^{-(t-4)} - e^{-(2t-8)} \right)</mrow>
          <mrow>y \amp  = e^{-t} - e^{-2t} + u_1(t) \left( e^{1-t} - e^{2-2t} \right) + u_2(t) \left( e^{2-t} - e^{4-2t} \right)</mrow>
          <mrow>\amp  \hspace{1cm} + u_3(t) \left( e^{3-t} - e^{6-2t} \right) + u_4(t) \left( e^{4-t} - e^{8-2t} \right)</mrow>
          <mrow>\amp  = \sum_{k=0}^\infty u_k(t) \left( e^{k-t} - e^{2(k-t)} \right)</mrow>
        </md>
      </p>
      <p>
        This is an interesting superposition of decay functions.
        They all have the same shape with a slightly higher peak.
        Adding them all up gives something which slowly rises higher and higher,
        while still trying to decay.
        Eventually the system does grow beyond any bounds,
        even with all the decay functions.
      </p>
    </statement>
  </example>
  <example>
    <statement>
      <p>
        This is an example with an integral.
        <md>
          <mrow>\frac{dy}{dt} + 6y(t) + 9 \int_0^t y(u) du \amp  = -1 \hspace{1cm} y(0) = 0</mrow>
          <mrow>sY+ 6Y + 9 \frac{Y}{s} \amp  = \frac{-1}{s}</mrow>
          <mrow>s^2 + 6sY + 9Y \amp  = -1</mrow>
          <mrow>Y \amp  = \frac{-1}{(s+3)^2} = \frac{d}{ds} \frac{1}{s+3}</mrow>
          <mrow>y \amp  = te^{-3t}</mrow>
        </md>
      </p>
      <p>
        We could try the previous example another way,
        by first differentiating both sides.
        <md>
          <mrow>\frac{dy}{dt} + 6y(t) + 9 \int_0^t y(u) du \amp  = -1 \hspace{1cm} y(0) = 0</mrow>
          <mrow>\frac{d^2y}{dt^2} + 6 \frac{dy}{dt} + 9y \amp  = 0</mrow>
          <mrow>r^2 + 6r + 9 \amp  = 0 \implies r = 3</mrow>
          <mrow>y \amp  = ae^{-3t} + bte^{-3t}</mrow>
          <mrow>y(0) \amp  = 0 \implies a=0</mrow>
          <mrow>y \amp  = bte^{-3t}</mrow>
        </md>
      </p>
    </statement>
  </example>
  <p>
    In this previous example, we would ask: what about <m>b</m>?
    In the original method, to match with the <m>-1</m>, we need <m>b=1</m>.
    In th second method,
    since we differentiated both sides of the equation,
    we lost the information that determined the constant <m>b</m>.
  </p>
</section>