<section xml:id="laplace-linear-odes">
  <title>Using Laplace Transforms to Solve Linear DEs</title>
  <p>
    As we've seen, Laplace transforms turn derivatives into algebraic operations.
    Therefore, particularly for certain linear equations,
    we can expect Laplace transforms to turn DEs into algebraic equations.
    We'll start with a very well known case:
    homogeneous second order constant coefficient linear equations.
  </p>
  <example>
    <statement>
      <me>
        y^{\prime \prime} + y = 0 \hspace{2cm} y(0) = 1 \hspace{1cm}
        y^\prime(0) = 0
      </me>
      <p>
        We apply the Laplace transform,
        making use of the initial values when we transform the derivative.
        <md>
          <mrow>\calL \{ y^{\prime \prime} + y \} \amp  = 0</mrow>
          <mrow>(s^2Y - sy(0) - y^\prime(0)) + Y \amp  = 0</mrow>
          <mrow>s^2Y - s + Y \amp  = 0</mrow>
          <mrow>(s^2+1)Y \amp  = s</mrow>
          <mrow>Y \amp  = \frac{s}{s^2 + 1}</mrow>
          <mrow>y \amp  = \calL^{-1} \left\{ \frac{s}{s^2+1} \right\} = \cos t</mrow>
        </md>
      </p>
      <p>
        We recover the expected <m>y(t) = \cos t</m>,
        but without any calculation of the characteristic equation or interpretation of complex roots.
        We also didn't have to get the complete solution and solve for unknown constants,
        since we made use of the initial values in the process.
        If initial values were not given,
        we would have to use unknown constants in their place in the calculation.
      </p>
    </statement>
  </example>
  <example>
    <statement>
      <p>
        Let's move on to a move involved harmonic system and assume that <m>b^2 - 4mk \lt  0</m>,
        so that we know to expect sinusoidal solutions.
        <me>
          my^{\prime \prime} + b y^\prime + ky = 0 \hspace{2cm} y(0) = 1 \hspace{1cm} y^\prime(0) = \frac{-b}{2m}
        </me>
      </p>
      <p>
        Then we can apply the Laplace transform to the entire equation.
        <md>
          <mrow>\calL \{ my^{\prime \prime} + b y^\prime + ky \} \amp  = \calL \{ 0 \}</mrow>
          <mrow>m (s^2Y - sy(0) - y^\prime(0)) + b(sY - y(0)) + kY \amp  = 0</mrow>
          <mrow>Y(ms^2 + bs + k) - ms - b + \frac{b}{2} \amp  = 0</mrow>
          <mrow>Y \amp  = \frac{ms+\frac{b}{2} }{ms^2+bs+k} = \frac{s + \frac{b}{2m}}{s^2 + \frac{b}{m} s + \frac{k}{m}}</mrow>
          <mrow>\amp  = \frac{s + \frac{b}{2m}}{ \left( s^2 + \frac{b}{m} s + \frac{b^2}{4m^2} \right)+ \left( \frac{k}{m} - \frac{b^2}{4m^2} \right) }</mrow>
          <mrow>\amp  = \frac{s + \frac{b}{2m}}{ \left( s + \frac{b}{2m} \right)^2 + \left( \frac{4km - b^2}{4m^2} \right)}</mrow>
          <mrow>y \amp  = \calL^{-1} \left\{ \frac{s + \frac{b}{2m}}{ \left( s + \frac{b}{2m} \right)^2 + \left( \frac{4mk - b^2}{4m^2} \right)} \right\}</mrow>
          <mrow>\amp  = e^{-\frac{b}{2m}t} \cos \left( \frac{\sqrt{4mk-b^2}}{2m} t \right)</mrow>
        </md>
      </p>
      <p>
        Now let's add a forcing term.
        Since we can take a Laplace transform of a delta function,
        we'll use that for the forcing term.
        <m>F\delta_0(t)</m> is a sudden impact with force <m>F</m>
        (in appropriate units)
        at time <m>t</m>.
        We'll use initial values of <m>y(0) = y^\prime(0) = 0</m>,
        so that the system is initially at rest.
        Again, we'll assume that <m>b^2 -4km \lt  0</m> for harmonic motion.
        <md>
          <mrow>my^{\prime \prime} + by^\prime + ky \amp  = F \delta_0(t)</mrow>
          <mrow>\calL \{ my^{\prime \prime} + by^\prime + ky \} \amp  = \calL \{ F \delta_0(t) \}</mrow>
          <mrow>m (s^2 Y - s y(0) - y^\prime(0)) + b(sY - y(0)) + kY \amp  = F</mrow>
          <mrow>(ms^2 + bs + k) Y \amp  = F</mrow>
          <mrow>Y \amp  = \frac{F}{ms^2 + bs + k}</mrow>
          <mrow>Y \amp  = \frac{\frac{F}{m}}{s^2 + \frac{b}{m}s + \frac{k}{m}}</mrow>
          <mrow>Y \amp  = \frac{\frac{F}{m}}{\left( s^2 + \frac{bs}{m} + \frac{b^2}{4m^2} \right) + \left( \frac{k}{m} - \frac{b^2}{4m^2} \right) }</mrow>
          <mrow>Y \amp  = \frac{F}{m} \frac{2m}{\sqrt{4km-b^2}} \frac{\frac{\sqrt{4km-b^2}}{2m}}{\left( s + \frac{b}{2m} \right)^2 + \left( \frac{4km - b^2}{4m^2} \right) }</mrow>
          <mrow>y(t) \amp  = \frac{2m}{4km-b^2} \frac{F}{m} e^{\frac{-b}{2m}t} \sin \left( \frac{\sqrt{4km-b^2}}{2m}t \right)</mrow>
          <mrow>y(t) \amp  = \frac{2F}{4km-b^2} e^{\frac{-b}{2m}t} \sin \left( \frac{\sqrt{4km-b^2}}{2m}t \right)</mrow>
        </md>
      </p>
      <p>
        We could ask:
        what changes if we move the impact to a later time?
        If the impact is at <m>t=4</m>,
        then the forcing term is <m>\delta_4(t)</m>.
        We again proceed with the Laplace transform.
        <md>
          <mrow>my^{\prime \prime} + by^\prime + ky \amp  = F \delta_4(t)</mrow>
          <mrow>\calL \{ my^{\prime \prime} + by^\prime + ky \} \amp  = \calL \{ F \delta_0(t) e^{-4s}\}</mrow>
          <mrow>m (s^2 Y - s y(0) - y^\prime(0)) + b(sY - y(0)) + kY \amp  = F e^{-4s}</mrow>
          <mrow>(ms^2 + bs + k) Y \amp  = F e^{-4s}</mrow>
          <mrow>Y \amp  = \frac{Fe^{-4s}}{ms^2 + bs + k}</mrow>
          <mrow>Y \amp  = \frac{\frac{Fe^{-4s}}{m}}{s^2 + \frac{b}{m}s + \frac{k}{m}}</mrow>
          <mrow>Y \amp  = e^{-4s} \frac{\frac{F}{m}}{\left( s^2 + \frac{bs}{m} + \frac{b^2}{4m^2} \right) + \left( \frac{k}{m} - \frac{b^2}{4m^2} \right) }</mrow>
          <mrow>Y \amp  = e^{-4s} \frac{F}{m} \frac{2m}{\sqrt{4km-b^2}} \frac{\frac{\sqrt{4km-b^2}}{2m}}{\left( s + \frac{b}{2m} \right)^2 + \left( \frac{4km - b^2}{4m^2} \right) }</mrow>
          <mrow>y(t) \amp  = u_4(t) \frac{2m}{4km-b^2} \frac{F}{m} e^{\frac{-b}{2m}(t-4)} \sin \left( \frac{\sqrt{4km-b^2}}{2m} (t-4) \right)</mrow>
          <mrow>y(t) \amp  = u_4(t) \frac{2F}{4km-b^2} e^{\frac{-b}{2m} (t-4) } \sin \left( \frac{\sqrt{4km-b^2}}{2m} (t-4) \right)</mrow>
        </md>
      </p>
      <p>
        Unsurprinsingly, we get precisely the same wave,
        just shifted <m>4</m> units to the right.
      </p>
    </statement>
  </example>
  <example>
    <statement>
      <p>
        This example has an exponential forcing term.
        <md>
          <mrow>y^{\prime \prime} + 4y^\prime + 4y \amp  = e^{-2t}</mrow>
          <mrow>y(0) \amp  = 0 \hspace{2cm} y^\prime(0) = 2</mrow>
          <mrow>s^2 Y - sy(0) - y^\prime(0) + 4(sY - y(0)) + 4Y \amp  = \frac{1}{s+2}</mrow>
          <mrow>s^2 Y - 2 + 4sY + 4Y \amp  = \frac{1}{s+2}</mrow>
          <mrow>(s^2 + 4s + 4)Y \amp  = \frac{1}{s+1} + 2 = \frac{2s+3}{s+2}</mrow>
          <mrow>Y \amp  = \frac{2s+3}{(s+2)(s+2)^2} = \frac{2s+3}{(s+2)^3}</mrow>
          <mrow>Y \amp  = \frac{2}{(s+2)^2} + \frac{1}{(s+2)^3}</mrow>
          <mrow>y \amp  = 2te^{-2t} + t^2e^{-2t} = e^{-2t}(2t+t^2)</mrow>
        </md>
      </p>
    </statement>
  </example>
  <example>
    <statement>
      <p>
        This example has a linear forcing term.
        <md>
          <mrow>y^{\prime \prime} + 4y \amp  = 4t^2 - 4t + 10</mrow>
          <mrow>y(0) \amp  = 0 \hspace{2cm} y^\prime(0) = 3</mrow>
          <mrow>s^2 Y - sy(0) - y^\prime(0) + 4Y \amp  = \calL \{ 4t^2 - 4t + 10 \}</mrow>
          <mrow>s^2 Y + 4sY -3 \amp  = \frac{8}{s^3} - \frac{4}{s^2} + \frac{10}{s}</mrow>
          <mrow>Y \amp  = \frac{8-4s+10s^2 + 3s^3}{s^3(s^2+4)}</mrow>
          <mrow>Y \amp  = \frac{2s^2-s+2}{s^3} + \frac{-2s+4}{s^2+4}</mrow>
          <mrow>\amp  = \frac{2}{s} - \frac{1}{s^2} + \frac{2}{s^3} - \frac{2s}{s^2+4} + \frac{4}{s^2+4}</mrow>
          <mrow>y \amp  = 2 - t + t^2 - 2 \cos 2t + 2 \sin 2t</mrow>
        </md>
      </p>
    </statement>
  </example>
  <example>
    <statement>
      <p>
        Since we can take Laplace transforms of piecewise-continuous functions,
        here is an example with a piecewise forcing term.
        <me>
          f(t) = \left\{ \begin{matrix} 0 \amp  t \leq \pi \\ 3 \cos t \amp  t > \pi \end{matrix} \right.
        </me>
      </p>
      <p>
        This represents a sinusoidal forcing term which is turned of at time <m>t=\pi</m>.
        We calculate the Lapalce transform of this piecewise function.
        <md>
          <mrow>y^{\prime \prime} + y \amp  = f(t) \hspace{2cm} y(0) = 0 \hspace{1cm} y^\prime(0) = 0</mrow>
          <mrow>s^2Y + Y \amp  = 3 \calL \{ u_\pi(t) \cos t\} = 3 \calL \{ -u_\pi(t) \cos (t-\pi) \}</mrow>
          <mrow>\amp  = -3 e^{-\pi s} \frac{s}{s^2+1}</mrow>
          <mrow>(s^2+1)Y \amp  = \frac{-3se^{-\pi s}}{s^2+1}</mrow>
          <mrow>Y \amp  = \frac{-3se^{-\pi s}}{(s^2+1)^2}</mrow>
          <mrow>Y \amp  = -3e^{-\pi s} \frac{s}{(s^2+1)^2}</mrow>
          <mrow>Y \amp  = -3e^{-\pi s} \frac{1}{2} \frac{d}{dt} \frac{-1}{s^2+1}</mrow>
          <mrow>y \amp  = \frac{-3}{2} u_{\pi}(t) (t-\pi) \sin (t-\pi)</mrow>
        </md>
      </p>
      <p>
        Notice that the forcing term is discontinuous,
        representing a sudden change,
        but the resulting solution is still continuous.
        The force suddenly changes, but the system still responds continuously.
      </p>
    </statement>
  </example>
</section>