<section xml:id="laplace-algebraic">
  <title>Algebraic Properties of the Laplace Transform</title>
  <p>
    We know that the Laplace transform is linear,
    but we said we would return to the issue of product.
    To start, it is easier to think in reverse:
    if we have a product <m>FG</m> in the <m>s</m>-domain,
    where did it come from in the <m>t</m>-domain?
    Here is the relevant calculation
    (the change in the order of integration near the end is jutified by theorems in multivariable analysis).
    <md>
      <mrow>FG \amp  = \int_0^\infty e^{-st} f(t) df \int_0^\infty e^{-su} g(t) du</mrow>
      <mrow>\amp  = \int_0^\infty \int_0^\infty e^{-s(u+t)} f(t)g(u) dt du</mrow>
      <mrow>\amp  = \int_0^\infty f(t) \left[ \int_0^\infty e^{-s(u+t)} g(u) du \right] du</mrow>
      <mrow>v \amp  = u+ t</mrow>
      <mrow>\amp  = \int_0^\infty f(t) \left[ \int_t^\infty e^{-sv} g(v-t) dv \right) dt</mrow>
      <mrow>\amp  = \int_0^\infty e^{-sv} \left[\int_0^t f(t) g(v-t) dt \right] dv</mrow>
      <mrow>\amp  = \calL \left\{ \int_0^t f(t) g(v-t) dt \right\}</mrow>
    </md>
  </p>
  <p>
    The product <m>FG</m> in the <m>s</m>-domain turns into this strange integral-based combination of the function <m>f</m> and <m>g</m>.
    This is a new <sq>product</sq>;
    it is called a convolution.
  </p>
  <definition>
    <statement>
      <p>
        Let <m>f,g</m> be integrable function on <m>[0,\infty)</m>.
        Their convoluiton is defined by this integral.
        <me>
          f \star g (t) = \int_0^t f(\tau) g(t-\tau) d \tau
        </me>.
      </p>
    </statement>
  </definition>
  <p>
    The convolution takes two functions and produces a new function,
    so it is a product.
    However, it is a strange product with new properties.
  </p>
  <proposition>
    <statement>
      <ul>
        <li>
          <p>
            The convolution is commutative:
            <m>f \star g = g \star f</m>.
          </p>
        </li>
        <li>
          <p>
            The convolution is associative:
            <m>(f \star g) \star h = f \star (g \star h)</m>.
          </p>
        </li>
        <li>
          <p>
            The convolution is distributive:
            <m>f \star (g \pm h) = f \star g \pm f \star h</m>.
          </p>
        </li>
        <li>
          <p>
            The convolution respect constants.
            <m>a (f \star g) = (af) \star g = f \star (ag)</m>
          </p>
        </li>
        <li>
          <p>
            The Laplace transform turns convolutions into products:
            <me>
              \calL \left\{ f \star g \right\} = F(s) G(s)
            </me>
          </p>
        </li>
      </ul>
    </statement>
  </proposition>
  <p>
    Here is an interesting question:
    if this is a product, what is the identity?
    That is, what function <m>g</m> satisfies
    <me>
      f \star g = \int_0^t f(\tau) g(t-\tau) d \tau = f(t)
    </me>.
  </p>
  <p>
    In this question,
    the integral needs to evaluate <m>f(\tau)</m> at <m>\tau = t</m>.
    We know a <sq>function</sq> that does this: <m>\delta_0</m>.
    <me>
      f \star \delta_0 = \int_0^t f(\tau) \delta_0 (t-\tau) d \tau = f(t)
    </me>
  </p>
  <proposition>
    <statement>
      <p>
        The <m>\delta</m>-function at 0 is the identity for the convolution.
      </p>
    </statement>
  </proposition>
  <p>
    The convolution behaves well with differentiation.
    <me>
      \frac{d}{dt} (f \star g) = \frac{df}{dt} \star g = g \star \frac{dg}{dt}
    </me>
  </p>
  <p>
    It also behaves well with integration.
    <me>
      \int_0^\infty f \star g dt = \int_0^\infty f(t) dt \int_0^\infty g(t) dt
    </me>
  </p>
  <p>
    Finally, it lets us understand inverse Lapalce transforms of products.
    <md>
      <mrow>\calL^{-t} \left\{ \frac{k^2}{(s^2+k^2)^2} \right\} \amp  = \calL^{-1} \left\{ \frac{k}{s^2+k^2} \frac{k}{s^2+k^2} \right\}</mrow>
      <mrow>\amp  = \sin kt \star \sin kt</mrow>
      <mrow>\amp  = \int_0^t \sin ku \sin (kt-ku) du</mrow>
      <mrow>\amp  \text{ Using }  \left[ \sin A \sin B = \frac{1}{2} \cos (A-B) - \cos (A+B) \right]</mrow>
      <mrow>\calL^{-t} \left\{ \frac{k^2}{(s^2+k^2)^2} \right\} \amp  = \frac{1}{2} \int_0^t \cos (ku - kt + ku) - \cos (ku + kt - ku ) du</mrow>
      <mrow>\amp  = \frac{1}{2} \int_0^t \cos (2ku - 2t) - \cos (kt) du</mrow>
      <mrow>\amp  = \frac{1}{2} \left. \frac{\sin (2ku - kt)}{2k} \right|_0^t - \left. \frac{1}{2} u \cos (kt) \right|_0^t</mrow>
      <mrow>\amp  = \frac{\sin (2kt-kt) - \sin (-kt)}{4k} - \frac{t\cos kt}{2}</mrow>
      <mrow>\amp  = \frac{\sin (kt)}{2k} - \frac{t\cos kt}{2} = \frac{\sin kt - kt \cos kt}{2k}</mrow>
    </md>
  </p>
  <p>
    In addition to differential equations,
    sometimes we get integral equations in mathematics.
    Laplace transforms and convolutions can help solve certain types of integral equations.
    <md>
      <mrow>3t^2 - e^{-t} - \int_0^t f(u) e^{t-u} du \amp  = f(t)</mrow>
      <mrow>3t^2 - e^{-t} - f \star e^t \amp  = f(t)</mrow>
      <mrow>\frac{6}{s^3} - \frac{1}{s+1} - F(s) \frac{1}{s-1} \amp  = F(s)</mrow>
      <mrow>\frac{6}{s^3} - \frac{1}{s+1} \amp  = F(s) \left( 1 + \frac{1}{s+1} \right)</mrow>
      <mrow>\frac{6}{s^3} - \frac{1}{s+1} \amp  = F(s) \left( \frac{s}{s-1} \right)</mrow>
      <mrow>F(s) \amp  = \frac{6(s-1)}{s^4} - \frac{(s-1)}{s(s+1)}</mrow>
      <mrow>\amp  = \frac{6}{s^3} - \frac{6}{s^4} + \frac{1}{s} - \frac{2}{s+1}</mrow>
      <mrow>f \amp  = 3t^2 - t^3 + 1 - 2e^{-t}</mrow>
    </md>
  </p>
</section>