<section xml:id="linear-des">
  <title>Linear Equations and Integrating Factors</title>
  <introduction>
    <p>
      First order linear equation have the general form
      <me>
        a(t) \frac{dy}{dt} + b(t) y = f(t)
      </me>.
    </p>
    <p>
      Here <m>a(t)</m>, <m>b(t)</m> and <m>f(t)</m> are various
      (usually continuous)
      functions.
      If we avoid the values where <m>a(t) = 0</m>,
      we can divide by <m>a(t)</m> to isolate the derivative,
      giving the following more typical form. (Remember the denominators!
      We have to pay attention to the roots of <m>a(t)</m> throughout the solution.)
      <me>
        \frac{dy}{dt} + P(t) y = Q(t)
      </me>
    </p>
  </introduction>
  <subsection xml:id="homogenoues">
    <title>Homogeneous Solutions</title>
    <p>
      The linear DE is called homogeneous if <m>Q(t) = 0</m>.
      In the homogeneous case,
      the DE is relatively easy to solve as a seperable equation.
      <md>
        <mrow>\frac{dy}{dt} \amp  = -P(t) y</mrow>
        <mrow>\frac{1}{y} dy \amp  = -P(t) dt</mrow>
        <mrow>\int \frac{1}{y} dy \amp  = -\int P(t) dt</mrow>
        <mrow>\ln |y| \amp  = -\int P(t) dt + c</mrow>
        <mrow>y \amp  = c e^{-\int P(t)} dt</mrow>
      </md>
    </p>
    <p>
      I should make a couple of notes about this calculation.
      <ul>
        <li>
          <p>
            We are informal with the constant.
            When we take exponents of each side of the equation,
            we should have multiplication by <m>e^c</m>.
            However, since this is still an undetermined constant,
            we simply write <m>c</m> instead of <m>e^c</m>.
            Also, when we drop the absolute value bars from <m>y</m>,
            we should have a <m>\pm</m> term.
            Again, since <m>c</m> can be either positive or negative,
            we don't worry about that <m>\pm</m>.
          </p>
        </li>
        <li>
          <p>
            We had a <m>y</m> in the denominator for this process,
            which means that we have to be careful at points where <m>y=0</m>.
            We use limits to figure out behaviour when <m>y</m> gets close to zero.
          </p>
        </li>
        <li>
          <p>
            If <m>P</m> is constant,
            this is our most basic exponential equation with solution <m>y = ce^{-\alpha t}</m>.
          </p>
        </li>
      </ul>
    </p>
  </subsection>
  <subsection xml:id="superposition">
    <title>Linear Operators and Superposition</title>
    <p>
      Recall from <xref ref="definition-linear-differential-operator">Definition</xref> the idea of linear operators.
      If we write <m>L = \frac{d}{dt} + P(t)</m>,
      we can write a second order DE as
      <me>
        L y = Q(t)
      </me>.
    </p>
    <p>
      This is a <em>linear</em> differential operator,
      so it behaves linearly, that is,
      it has the two linearity properties.
      <md>
        <mrow>L(y_1 + y_2) \amp  = Ly_1 + Ly_2</mrow>
        <mrow>L(cy) \amp  = cL(y)</mrow>
      </md>
    </p>
    <p>
      Then consider both the homoegenous equation <m>Ly = 0</m> and a non-homogenous equation <m>Ly = Q(t)</m>.
      If <m>f</m> is a solution to the non-homogenous equation,
      then <m>Lf = Q(t)</m>,
      and if <m>g</m> is a solution to the homogenous equation,
      then <m>Lg = 0</m>.
      By linearity, we can conclude that
      <me>
        L(f+\alpha g) = Lf + \alpha Lg = Q(t) + \alpha \cdot 0 = Q(t)
      </me>.
    </p>
    <definition>
      <statement>
        <p>
          If we have a solution to <m>Ly=Q(t)</m>,
          we can get other solutions by adding multiples of the solution to the homogeneous equation <m>Ly=0</m>.
          The solution to <m>Ly = Q(t)</m> is called the
          <term>particular solution</term>
          and this process is called <term>superposition of solutions</term>.
        </p>
      </statement>
    </definition>
    <p>
      For those who remember their linear algebra,
      we can think of the solutions of a linear equation as a linear subspace of the vector space of differentiable functions
      (on an appropriate domain).
      In this sense the solution set of a linear equation is an offset span:
      the non-homogenous solution is the offset and the basis of the span is any homogenous solution.
      Superposition gives us the family-structure of solutions to linear equations.
      Any multiple of a homogenous solutions can be added to the particular solution,
      so the family is the particular solution plus any multiple of a homogeneous solutions:
      <m>y_p + \alpha y_h</m>.
      This <m>\alpha</m> is the parameter of the family.
    </p>
  </subsection>
  <subsection xml:id="integrating-factors">
    <title>Integrating Factors</title>
    <p>
      We know how to solve homogenous linear equations, since they are seperable.
      Finding non-homogenous solutions is somewhat more difficult;
      since these are not seperable equations, we need a new technique.
    </p>
    <p>
      Let <m>L = \frac{d}{dt} + Q(t)</m> be as before,
      and let <m>y_h</m> be a homogeneous solutions (a solution to <m>Ly = 0</m>).
      The technique we will use is called
      <em>variation of parameters</em>.
      This technique says we should look for a particular solution of the type <m>y_p = g(t) y_h</m>.
      Assuming that our solution has this special form,
      we have to try to find this <m>g(t)</m>.
      In order to do that, we put <m>g(t) y_h</m> into the equation.
      <md>
        <mrow>Ly_p(t) = L g(t) y(t) \amp  = Q(t)</mrow>
        <mrow>g^\prime(t) y(t) + g(t) y^\prime(t) + g(t) P(t) y(t) \amp  = Q(t)</mrow>
        <mrow>g^\prime(t) y(t) + g(t) \Big( y^\prime(t) + P(t) y(t) \Big) = g^\prime(t) + g(t) L y \amp  = Q(t)</mrow>
        <mrow>g^\prime(t) y(t) + g(t) 0 \amp  = Q(t)</mrow>
        <mrow>g^\prime(t) \amp  = \frac{Q(t)}{y(t)}</mrow>
        <mrow>g(t) \amp  = \int \frac{Q(t)}{y(t)}</mrow>
      </md>
    </p>
    <p>
      We can put this back into our special form and use the fact that the homogeneous solution is <m>y = e^{-\int P(t)dt}</m>.
      <md>
        <mrow>y_p = g(t) y \amp  = \left( \int \frac{Q(t)}{e^{-\int P(t) dt}} dt \right) e^{-\int P(t) dt }</mrow>
        <mrow>y_p \amp  = e^{-\int P(t) dt} \int e^{\int P(t) dt} Q(t) dt</mrow>
      </md>
    </p>
    <definition>
      <statement>
        <p>
          In solving a linear equation of the for <m>\frac{dy}{dt} + P(t) y = Q(t)</m>,
          the expression <m>e^{\int P(t) dt}</m> is called an
          <term>integrating factor</term>
          and it is typically written <m>\mu(t)</m>.
        </p>
      </statement>
    </definition>
    <p>
      We rearrange the expression using the integrating factor.
      <md>
        <mrow>e^{\int P(t) y} y_p \amp  = \int e^{\int P(t) dt} Q(t) dt</mrow>
        <mrow>\frac{d}{dt} \left( e^{\int P(t) dt} y_p \right) \amp  = e^{\int P(t) dt} Q(t)</mrow>
        <mrow>\frac{d}{dt} (\mu (t) y_p(t)) \amp  = \mu (t) Q(t)</mrow>
        <mrow>y_p \amp  = \frac{\int \mu(t) Q(t) dt + c}{\mu (t)}</mrow>
      </md>
    </p>
    <p>
      Multiplying by the integrating factor turns the
      <m>y_p^\prime(t) + P(t) y_p(t)</m> side of the equation into a product rule derivative,
      which we can just integrate to solve.
      The integrating factor turns a linear equation into something that can be directly solved by integration,
      hence the name.
      It is best to remember the process this way:
      the original DE becomes a product rule derivative problem by multiplying both sides of the original DE by the integrating factor and then isolating <m>y_p</m>.
    </p>
    <p>
      This variation of parameters is the first instance of a very common approach to solving DEs.
      Often, working with no idea of what kind of function we are looking for is simply too open-ended and too difficult.
      Therefore, we make a reasonable guess regarding the form of the solution.
      Here, that guess was <m>y_p = g(t) y_h</m> where <m>g(t)</m> was some unknown function.
      Then we put out special form back into the DE and try to find specific information about the parameter or unknown involved.
    </p>
  </subsection>
  <subsection xml:id="linear-equations-examples">
    <title>Examples</title>
    <example xml:id="linear-example1">
      <statement>
        <me>
          \frac{dy}{dt} + \frac{y}{t} = 2e^t
        </me>
        <p>
          Since there is a <m>t</m> in the denominator,
          we must avoid <m>t=0</m> in the domain of solutions.
          We first look for the homogeneous solution.
          <me>
            y_h(t) = ce^{-\int \frac{1}{t}} dt = ce^{-\ln |t|} = \frac{c}{t}
          </me>
        </p>
        <p>
          Then the integrating factor is
          <me>
            \mu(t) = e^{\int \frac{1}{t} dt } = e^{\ln |t|} = t
          </me>.
        </p>
        <p>
          We use the integrating factor to get a new DE.
          <md>
            <mrow>\mu(t) \frac{dy}{dt} + \mu(t) \frac{y}{t} \amp  = \mu(t) 2e^t</mrow>
            <mrow>t \frac{dy}{dt} + t \frac{y}{t} \amp  = t 2e^t</mrow>
            <mrow>\frac{d}{dt} (t y) \amp  = 2te^t</mrow>
            <mrow>ty \amp  = \int (2te^t) dt</mrow>
            <mrow>ty \amp  = 2(te^t - e^t) + c</mrow>
            <mrow>y \amp  = 2 \left( e^t - \frac{e^t}{t} \right) + \frac{c}{t}</mrow>
          </md>
        </p>
        <p>
          Notice that we actually get the the homogeneous pieces here from the constant of integration,
          getting the whole linear family.
          Also notice that <m>t=0</m> is excluded from the domain.
        </p>
      </statement>
    </example>
    <example>
      <statement>
        <me>
          (t^2-9) \frac{dy}{dt} + ty = 0
        </me>
        <p>
          This is just a homogeneous DE. We note that <m>t \neq \pm 3</m> in the domain.
          The solution to the homogeneous case is
          <me>
            y = e^{-\int P(t) dt} = e^{-\int \frac{t}{t^2-9} dt} = e^{ - \frac{1}{2} \ln |t^2-9| + c} = \frac{c}{\sqrt{t^2-9}}
          </me>.
        </p>
        <p>
          We should be careful with the absolute value in <m>\ln |f(t)|</m>.
          The calculation can be done in two pieces,
          when <m>f(t) > 0</m> and when <m>f(t) \lt 0</m>.
          In the previous calculation, we were a little careless with this detail.
        </p>
      </statement>
    </example>
    <example>
      <statement>
        <me>
          \frac{dy}{dt} + y = f(t)
        </me>
        <p>
          To add some complication,
          the non-homogeneous function here is going to be a step function.
          <me>
            f(t) = \left\{ \begin{matrix} 1 \amp  0 \leq t \leq 1 \\ 0 \amp  t > 1 \end{matrix} \right.
          </me>
        </p>
        <p>
          This is still allowed:
          often the coefficients and functions involved in DEs are only piecewise continuous and/or piecewise differentiable.
          We can still work with them.
          The integrating factor is <m>\mu(t) = e^{\int 1 dt} = e^t</m>.
          We have to work with two different intervals.
          First look at <m>[0,1]</m>.
          <me>
            \frac{d}{dt} e^t y = e^t \implies e^ty = e^t + c_1 \implies y = 1 + c_1e^{-t}
          </me>
        </p>
        <p>
          Alternatively, look at <m>(1,\infty)</m>.
          <me>
            \frac{d}{dt} e^t y = 0 \implies e^ty = t + c_2 \implies y = c_2e^{-t}
          </me>
        </p>
        <p>
          We have two constants, but we want a continuous solution.
          (It will fail to be differentiable at <m>t=1</m>, but that's alright.
          There is a sudden change in the situation, so that's expected.)
          Continuity at <m>1</m> means that <m>e-c_1 = c_2</m>.
          The final solution is a continuous piecewise function.
          <me>
            y = \left\{ \begin{matrix} 1 - ce^{-t} \amp  t \in [0,1] \\ (e-c)e^{-t} \amp  t \in (1,\infty) \end{matrix} \right.
          </me>
        </p>
        <p>
          Even with this piecewise function,
          we can still do initial value problems.
          If <m>y(0) =0</m>,
          we find that <m>c=1</m> and we get a specific solution.
        </p>
      </statement>
    </example>
  </subsection>
</section>