<section xml:id="linear-systems">
  <title>Linear Systems</title>
  <subsection xml:id="qualitative-analysis">
    <title>Qualitative Analysis</title>
    <p>
      A linear system of two differential equations has the form
      <md>
        <mrow>x^\prime \amp  = ax + by</mrow>
        <mrow>y^\prime \amp  = cx + dx</mrow>
      </md>.
    </p>
    <p>
      The nullclines of a linear system are the lines
      <m>y = \frac{-a}{b} x</m> and <m>y = \frac{-c}{d}</m>.
      The only steady state is <m>(0,0)</m>.
      The six behaviours listed in the previous section (stable/unstable node,
      stable/unstable focus, saddle, centre) are all possible.
      However, for linear systems,
      these six cases are the <em>only</em> possible cases.
    </p>
  </subsection>
  <subsection xml:id="laplace-linear-systems">
    <title>Laplace Transforms for Linear Systems</title>
    <figure xml:id="figure-linear-system1">
      <caption>First Linear System Example</caption>
      <image width="800%" source="images/figure39.png" />
    </figure>
    <example>
      <statement>
        <p>
          Let's start with a simple example.
          We can solve linear systems with Laplace transforms,
          since the Laplace transform will be a linear system of algebraic
          (not differential)
          equations.
          We solve these with basic techniques,
          such as isolating and replacing, or with linear algebra.
          <md>
            <mrow>x^\prime \amp  = -y</mrow>
            <mrow>y^\prime \amp  = x</mrow>
            <mrow>x(0) \amp  = 0 \hspace{1cm} y(0) = 1</mrow>
            <mrow>sX \amp  = -Y \implies X = \frac{-Y}{s}</mrow>
            <mrow>sY -1 \amp  = X \implies sY - 1 = \frac{-Y}{S}</mrow>
            <mrow>sY + \frac{Y}{s} \amp  = 1</mrow>
            <mrow>Y \amp  = \frac{s}{s^2+1}</mrow>
            <mrow>X \amp  = \frac{-Y}{s} = \frac{-1}{s^2+1}</mrow>
            <mrow>y \amp  = \cos t</mrow>
            <mrow>x \amp  = - \sin t</mrow>
          </md>
        </p>
        <p>
          In this case, the nullclines are simply the axes.
          The steady state <m>(0,0)</m> is a centre.
          <xref ref="figure-linear-system1">Figure</xref>
          shows the nullclines and directions.
        </p>
      </statement>
    </example>
    <figure xml:id="figure-linear-system2">
      <caption>Second Linear System Example</caption>
      <image width="800%" source="images/figure35.png" />
    </figure>
    <example>
      <statement>
        <md>
          <mrow>x^\prime \amp  = 2x + 2y \hspace{1cm} x(0) = 1</mrow>
          <mrow>y^\prime \amp  = 2x - y \hspace{1.2cm} y(0) = 1</mrow>
          <mrow>sX - 1 \amp  = 2X + 2Y</mrow>
          <mrow>sY - 1 \amp  = 2X - Y \implies X = \frac{2Y+1}{s-2}</mrow>
          <mrow>sY - 2 \left( \frac{2Y+1}{s-2} \right) + Y \amp  = 1</mrow>
          <mrow>(s+1) Y - \frac{4Y}{s-2} \amp  = 1 + \frac{2}{s-2}</mrow>
          <mrow>\left( \frac{s^2-s-6}{s-2} \right) Y \amp  = 1 + \frac{2}{s-2}</mrow>
          <mrow>Y \amp  = \frac{s-2}{(s-3)(s+2)} + \frac{2}{(s-3)(s+2)} =
          \frac{s}{(s-3)(s+2)}</mrow>
          <mrow>\amp  = \frac{\frac{2}{5}}{s+2} + \frac{\frac{3}{5}}{s-3}</mrow>
          <mrow>X \amp  = \frac{2Y+1}{s-2} = \frac{2\left( \frac{s}{(s-3)(s+2)}
          \right) + 1}{s-2} = \frac{2s + s^2 - s - 6}{(s-3)(s-2)(s+2)}</mrow>
          <mrow>\amp  = \frac{(s+3)(s-2)}{(s-3)(s-2)(s+2)}
          = \frac{s+3}{(s-3)(s+2)} = \frac{\frac{6}{5}}{s-3} -
          \frac{\frac{1}{5}}{s+2}</mrow>
          <mrow>x \amp  = \frac{6}{5} e^{3t} - \frac{1}{5} e^{-2t}</mrow>
          <mrow>y \amp  = \frac{2}{5} e^{-2t} + \frac{3}{5} e^{3t}</mrow>
        </md>
        <p>
          In this case,
          the nullclines are <m>y = -x</m> and <m>y = 2x</m>.
          The steady state is a saddle point.
          The solutions are a mix of exponential growth and exponential decay;
          this mix of growth and decay fits the expected behaviour of a saddle point.
          <xref ref="figure-linear-system2">Figure</xref>
          shows the nullclines and directions.
        </p>
      </statement>
    </example>
    <figure xml:id="figure-linear-system3">
      <caption>Third Linear System Example</caption>
      <image width="600%" source="images/figure36.png" />
    </figure>
    <example>
      <statement>
        <md>
          <mrow>x^\prime \amp  = 2x + 3y \hspace{1cm} x(0) = 1</mrow>
          <mrow>y^\prime \amp  = 2x + y \hspace{1.2cm} y(0) = 1</mrow>
          <mrow>sX - 1 \amp  = 2X + 3Y</mrow>
          <mrow>sY - 1 \amp  = 2X + Y \implies X = \frac{3Y+1}{s-2}</mrow>
          <mrow>sY - Y - 2 \left( \frac{3Y+1}{s-2} \right) \amp  = 1</mrow>
          <mrow>\left( \frac{s^2-3s-4}{s-2} \right) Y \amp  = 1 + \frac{2}{s-2}</mrow>
          <mrow>Y \amp  = \frac{s-2}{(s-4)(s+1)} + \frac{2}{(s-4)(s+1)} =
          \frac{s}{(s-4)(s+1)} = \frac{\frac{4}{5}}{s-4} +
          \frac{\frac{-1}{5}}{s+1}</mrow>
          <mrow>X \amp  = \frac{3\frac{s}{(s-4)(s+1)} + 1}{s-2} =
          \frac{3s+s^2-3s-4}{(s+1)(s-4)(s-2)} =
          \frac{s^2-4}{(s+1)(s-4)(s-2)}</mrow>
          <mrow>\amp  = \frac{s+2}{(s+1)(s-4)} = \frac{\frac{6}{5}}{s-4} -
          \frac{\frac{1}{5}}{s+1}</mrow>
          <mrow>x \amp  = \frac{6}{5} e^{4t} - \frac{1}{5} e^{-t}</mrow>
          <mrow>y \amp  = \frac{4}{5} e^{4t} + \frac{1}{5} e^{-t}</mrow>
        </md>
        <p>
          In this case,
          the nullclines are <m>y = \frac{-2}{3}x</m> and <m>y = -2x</m>.
          The behaviour is again a saddle point and again we have a mix of positive and negative exponential terms.
          <xref ref="figure-linear-system3">Figure</xref>
          shows the nullclines and directions.
        </p>
      </statement>
    </example>
    <figure xml:id="figure-linear-system4">
      <caption>Fourth Linear System Example</caption>
      <image width="700%" source="images/figure37.png" />
    </figure>
    <example>
      <statement>
        <md>
          <mrow>x^\prime \amp  = 3x - 18y \hspace{1cm} x(0) = 1</mrow>
          <mrow>y^\prime \amp  = 2x - 9y \hspace{1.2cm} y(0) = 1</mrow>
          <mrow>sX - 1 \amp  = 3X - 18Y</mrow>
          <mrow>sY - 1 \amp  = 2X - 9Y \implies X = \frac{1-18Y}{s-3}</mrow>
          <mrow>sY + 9Y - 2 \left( \frac{1-18Y}{s-3} \right) \amp  = 1</mrow>
          <mrow>\left( \frac{s^2+6s+9}{s-3} \right) Y \amp  = 1 + \frac{2}{s-3}</mrow>
          <mrow>Y \amp  = \frac{s-3}{(s+3)^2} + \frac{2}{(s+3)^2} =
          \frac{s-1}{(s+1)^2}</mrow>
          <mrow>\amp  = \frac{s}{(s+3)^2} - \frac{1}{(s+3)^2}
          = \frac{1}{s+3} - \frac{4}{(s+3)^2}</mrow>
          <mrow>X \amp  = \frac{1 - 19 \frac{s-1}{(s+3)^2}}{s-3} =
          \frac{s^2-12s+27}{(s-3)(s+3)^2}
          \frac{(s-9)(s-3)}{(s-3)(s+3)^2}</mrow>
          <mrow>\amp  = \frac{s}{(s+3)^2} - \frac{1}{(s-3)^2} = \frac{1}{s+3} -
          \frac{12}{(s+3)^2}</mrow>
          <mrow>x \amp  = e^{-3t} + 12 t e^{-3t}</mrow>
          <mrow>y \amp  = e^{-3t} + 4 t e^{-3t}</mrow>
        </md>
        <p>
          In this case, the nullclines are
          <m>y = \frac{1}{6}x</m> and <m>y = \frac{2}{9}x</m>.
          The steady state is a stable focus.
          The solutions are all decay terms,
          so they all tend to the steady state.
          This doesn't really match the expected behaviour,
          which looks like rotation.
          This is an interesting example:
          the repeated factor leads to the <m>t e^{-3t}</m> terms,
          which do have more spinning motion that the general exponential terms.
          This is like the critically damped case for harmonic motion:
          it is very close to sinusoidal behaviour but not quite there.
          It would be very easy to interpret the trajectories as rotational;
          in this case, the qualitative analysis is misleading.
          <xref ref="figure-linear-system4">Figure</xref>
          shows the nullclines and directions.
        </p>
      </statement>
    </example>
    <figure xml:id="figure-linear-system5">
      <caption>Fifth Linear System Example</caption>
      <image width="600%" source="images/figure38.png" />
    </figure>
    <example>
      <statement>
        <md>
          <mrow>x^\prime \amp  = 6x - y \hspace{1.2cm} x(0) = 1</mrow>
          <mrow>y^\prime \amp  = 5x + 4y \hspace{1cm} y(0) = 1</mrow>
          <mrow>sX - 1 \amp  = 6X - Y</mrow>
          <mrow>sY - 1 \amp  = 5X + 4Y \implies X = \frac{1-Y}{s-6}</mrow>
          <mrow>(s-4)Y - 5 \left( \frac{1-y}{s-6} \right) \amp  = 1</mrow>
          <mrow>\left( \frac{s^2-10s+29}{s-6} \right) Y \amp  = 1 - \frac{5}{s-6}
          = \frac{s-11}{s-6}</mrow>
          <mrow>Y \amp  = \frac{s-11}{s^2-10s_29} = \frac{s}{(s-5)^2+4} -
          \frac{11}{(s-5)^2 + 4}</mrow>
          <mrow>\amp  = \frac{s-5}{(s-5)^2+4} - \frac{6}{(s-5)^2 + 4}</mrow>
          <mrow>X \amp  = \frac{1 - \frac{s-11}{s^2+10s+29}}{s-6} =
          \frac{s^2-11s + 40}{(s-6)(s^2-10s+29)} =
          \frac{(s-6)(s-5)}{(s-6)(s^2-10s+19)}</mrow>
          <mrow>\amp  = \frac{s-5}{s^2-10s+29} = \frac{s-5}{(s-5)^2 +4} -
          \frac{1}{(s-5)^2 + 4}</mrow>
          <mrow>x \amp  = e^{5t} \cos 2t - 3 e^{5t} \sin 2t</mrow>
          <mrow>y \amp  = e^{5t} \cos 2t - \frac{1}{2} e^{5t} \sin 2t</mrow>
        </md>
        <p>
          In this case,
          the nullclines are <m>y = 6x</m> and <m>y = \frac{-5}{4}x</m>.
          The steady state is unstable node.
          The solutions have rotation in the sinusoidal terms and exponential growth,
          showing the outward spiral expected from an unstable node.
          <xref ref="figure-linear-system5">Figure</xref>
          shows the nullclines and trajectories for this example.
        </p>
      </statement>
    </example>
  </subsection>
  <subsection xml:id="second-order-systems">
    <title>Second Order Systems</title>
    <p>
      We used coupled spring as a motivating example is a linear system.
      It is a second order system<ndash/>in fact,
      it will be the only example we'll consider of a second order system.
      <md>
        <mrow>m_1x_1^{\prime \prime} \amp  = - k_1x_1 + k_2(x_2 - x_1)</mrow>
        <mrow>m_2x_2^{\prime \prime} \amp  = -k_2(x_2-x_1)</mrow>
      </md>
    </p>
    <p>
      Let's set the constants <m>m_1 = m_2 =1</m>,
      <m>k_1=8</m> and <m>k_2=3</m>.
      Let's also set the initial conditions <m>x_1(0) = x_1^\prime(0) = 0</m> and
      <m>x_2(0) = 1</m> and <m>x_2^\prime(0) = 0</m>.
      These initial condition implies that we've pushed <m>x_2</m> away from equilibrium.
      We don't have a phase-plane diagram here,
      since this is a second order system.
      (Our phase-plane diagram intepretation in the previous section was specific to first-order systems.)
    </p>
    <p>
      We solve using Laplace transforms.
      <md>
        <mrow>x_1^{\prime \prime} + 11 x_1 - 3x_2 \amp  = 0</mrow>
        <mrow>x_2^{\prime \prime} + 3 x_2 - 3x_1 \amp  = 0</mrow>
        <mrow>s^2 X_1 + 11 X_1 - 3X_2 \amp  = 0</mrow>
        <mrow>s^2 X_2 - s + 3X_2 - 3X_1 \amp  = 0</mrow>
        <mrow>X_2 \amp  = \frac{(s^2+11) X_1}{3}</mrow>
        <mrow>(s^2+3)X_2 - 3X_1 \amp  = s</mrow>
        <mrow>(s^2+3)\left( \frac{s^2+11}{3} \right) - 3X_1 \amp  = s</mrow>
        <mrow>\frac{s^4 + 14s^2+ 33 - 9}{3} X_1 \amp  = s</mrow>
        <mrow>\frac{s^4 + 14s^2 + 24}{3} X_1 \amp  = s</mrow>
        <mrow>X_1 \amp  = \frac{3x}{s^4 + 14s^2 + 24} = \frac{3s}{(s^2+2)(s^2+12)}</mrow>
        <mrow>X_2 \amp  = \frac{s^2+11}{3} \frac{3s}{(s^2+2)(s^2+12)} = \frac{s^3 + 11s}{(s^2+1)(s^2+12)}</mrow>
        <mrow>X_1 \amp  = \frac{3s}{10(s^2+2)} - \frac{3s}{10(s^2+12)}</mrow>
        <mrow>X_2 \amp  = \frac{9s}{10(s^2+2)} + \frac{s}{10(s^2+12)}</mrow>
        <mrow>x_1 \amp  = \frac{3}{10} \cos \sqrt{2}t - \frac{3}{10} \cos \sqrt{12} t</mrow>
        <mrow>x_2 \amp  = \frac{9}{10} \cos \sqrt{2}t + \frac{1}{10} \cos \sqrt{12} t</mrow>
      </md>
    </p>
    <p>
      Here is an adjustment of the coupled spring,
      where each mass is attached to a fixed object.
      Then there are three springs in total:
      one attaching each mass to opposite walls, and one between them.
      We have a system given by Newton's laws of motion.
      <md>
        <mrow>m_2 x^{\prime \prime} \amp  = -k_1 x + k_2 (y-x)</mrow>
        <mrow>m_2 y^{\prime \prime} \amp  = -k_3 y + k_2 (x-y)</mrow>
      </md>
    </p>
    <p>
      We set the constants <m>k_1 = k_3 = 2</m>,
      <m>k_2 = 1</m>, and <m>m_1 = m_2 = 1</m>.
      For initial conditions, we set <m>x(0) = y(0) = 0</m> and
      <m>x^\prime(0) = -1</m>, <m>y^\prime(0) = 1</m>.
      These initial contidions show that,
      the masses are pushed apart equal distances to start the system.
      <md>
        <mrow>x^{\prime \prime} + 3x - y \amp  = 0</mrow>
        <mrow>y^{\prime \prime} + 3y - x \amp  = 0</mrow>
        <mrow>s^2X + 1 + 3X - Y \amp  = 0</mrow>
        <mrow>s^2Y - 1 + 3Y - X \amp  0</mrow>
        <mrow>Y \amp  = \frac{1++X}{s^2+3}</mrow>
        <mrow>(s^2+3) X - \left( \frac{1+X}{s^2+3} \right) \amp  = - 1</mrow>
        <mrow>\left( \frac{(s^2+3)(s^2+3) - 1}{s^2+3)} \right) X \amp  = \frac{1}{s^2+3} - 1</mrow>
        <mrow>(s^4+6s^2+8)X \amp  = -s^2-2</mrow>
        <mrow>X \amp  = \frac{-s^2-2}{(s^2+4)(s^2+2)} = \frac{-1}{s^2+4}</mrow>
        <mrow>Y \amp  = \frac{1 + \frac{-1}{s^2+4}}{s^2+3}</mrow>
        <mrow>\amp  = \frac{s^2+4-1}{(s^2+4)(s^2+3)}</mrow>
        <mrow>\amp = \frac{s^2+3}{(s^2+4)(s^2+3)} = \frac{1}{s^2+4}</mrow>
        <mrow>x \amp  = -\sin 2t</mrow>
        <mrow>y \amp  = \sin 2t</mrow>
      </md>
    </p>
  </subsection>
  <subsection xml:id="general-theory">
    <title>General Theory via Eigenvalues</title>
    <p>
      The general linear system with two equations has the form
      <me>
        x^\prime = ax + by \hspace{1cm} y^\prime = cx + dy
      </me>.
    </p>
    <p>
      We can use a 2 by 2 matrix with coefficients <m>a,b,c,d</m> to analyze the behaviour.
      We were <m>x</m> and <m>y</m> as the coordinates of a vector.
      <me>
        \left[ \begin{matrix} x_1^\prime \\ x_2^\prime \end{matrix} \right] = \left[ \begin{matrix} a \amp  b \\ c \amp  d \end{matrix} \right] \left[ \begin{matrix} x_1 \\ x_2 \end{matrix} \right]
      </me>
    </p>
    <p>
      Let <m>v</m> be an eigenvectors of the matrix and let <m>\lambda</m> be the corresponding eigenvectors.
      <me>
        \left[ \begin{matrix} x_1 \amp  x_2 \end{matrix} \right] = e^{\lambda t} v = \left[ \begin{matrix} e^{\lambda t} v_1 \\ e^{\lambda t} v_1 \end{matrix} \right]
      </me>
    </p>
    <p>
      To see why this is a solution,
      see what happens when the matrix acts on the vector.
      <md>
        <mrow>\left[ \begin{matrix} a \amp  b</mrow>
        <mrow>c \amp  d \end{matrix} \right] \left[ \begin{matrix} e^{\lambda t} v_1</mrow>
        <mrow>e^{\lambda t} v_2 \end{matrix} \right] \amp  = e^{\lambda t} \left[ \begin{matrix} a \amp  b</mrow>
        <mrow>c \amp  d \end{matrix} \right] \left[ \begin{matrix} v_1</mrow>
        <mrow>v_2 \end{matrix} \right] = e^{\lambda t} \lambda \left[ \begin{matrix} v_1</mrow>
        <mrow>v_2 \end{matrix} \right] = \left[ \begin{matrix} \lambda e^{\lambda t} v_1</mrow>
        <mrow>\lambda e^{\lambda t} v_2 \end{matrix} \right]</mrow>
        <mrow>[1em] \amp  = \left[ \begin{matrix} \dfrac{d}{dt}e^{\lambda t} v_1</mrow>
        <mrow>[1em] \dfrac{d}{dt} e^{\lambda t} v_2 \end{matrix} \right] = \frac{d}{dt} \left[ \begin{matrix} e^{\lambda t} v_1</mrow>
        <mrow>e^{\lambda t} v_2 \end{matrix} \right]</mrow>
      </md>
    </p>
    <p>
      If we allow for complex eigenvalues,
      the matrix has two eigenvalues,
      wth two linearly independent eigenvectors,
      giving two linearly independent solutions of this type.
      If the eigenvalues are real, there are exponential growth/decay solutions.
      If the eigenvalues are complex,
      these are sinusoidal solutions.
    </p>
  </subsection>
  <subsection xml:id="stability-eigenvalues">
    <title>Stability via Eigenvalues</title>
    <p>
      Everything about a linear system can be determined by the eigenvalues of the associated matrix.
      For a linear system, the nullclines are both lines through the origin.
      Assuming they are not the same line
      (which would make the system redundant),
      the only steady state for a linear system in two equations is <m>(0,0)</m>.
      As we've stated previously,
      there are six behaviours at the steady state for two-dimensional linear systems:
      stable and unstable foci, stable and unstable notes, centres and saddles.
      We can identify each case simply by the eigenvalues.
      <ul>
        <li>
          <p>
            If both eigenvalues are real and negative,
            then <m>(0,0)</m> is a stable node.
          </p>
        </li>
        <li>
          <p>
            If both eigenvalues are real and positive,
            then <m>(0,0)</m> is a unstable node.
          </p>
        </li>
        <li>
          <p>
            If both eigenvalues are real,
            but one is positive and one is negative,
            then <m>(0,0)</m> is a saddle point.
          </p>
        </li>
        <li>
          <p>
            If both eigenvalues are complex with negative real part,
            then <m>(0,0)</m> is a stable focus.
          </p>
        </li>
        <li>
          <p>
            If both eigenvalues are complex with positive real part,
            then <m>(0,0)</m> is an unstable focus.
          </p>
        </li>
        <li>
          <p>
            If both eigenvalues are complex and purely imaginary,
            then <m>(0,0)</m> is a centre.
          </p>
        </li>
      </ul>
    </p>
    <p>
      The eigenvalues become the coefficients of the exponential solutions,
      which explains this list of behaviours.
      Only when we have complex coefficients do we get sinusoidal behaviuors,
      as in the spiral foci and the circular centre.
      When we have real coefficients,
      we only get growth and decay.
      The real part, in either case,
      is the growth or decay term.
      When the real part is negative,
      we have decay, which is stability.
      When the real part is positive,
      we have growth, which is instability.
    </p>
    <p>
      Let <m>M</m> be the matrix and let Let
      <m>\alpha = \text{ tr } M</m> and <m>\beta = \det M</m>.
      Then the characteristic equation of the matrix can be written <m>\lambda^2 - \alpha \lambda + \beta = 0</m>.
      In addition,
      let <m>\delta</m> be the discriminant of the characteristic polynomial,
      <m>\delta = \alpha^2 - 4\beta</m>.
      Then we can redo the previous list.
      <ul>
        <li>
          <p>
            If <m>\beta > 0</m>, <m>\alpha \lt 0</m> and
            <m>\delta > 0</m> then <m>(0,0)</m> is a stable node.
          </p>
        </li>
        <li>
          <p>
            If <m>\beta > 0</m>, <m>\alpha > 0</m> and <m>\delta > 0</m>,
            then <m>(0,0)</m> is an unstable node.
          </p>
        </li>
        <li>
          <p>
            If <m>\beta \lt 0</m>, then <m>(0,0)</m> is a saddle point.
          </p>
        </li>
        <li>
          <p>
            If <m>\beta > 0</m>, <m>\alpha \lt 0</m> and <m>\delta \lt 0</m>,
            then <m>(0,0)</m> is a stable focus.
          </p>
        </li>
        <li>
          <p>
            If <m>\beta > 0</m>, <m>\alpha> 0</m> and
            <m>\delta \lt 0</m> then <m>(0,0)</m> is an unstable focus.
          </p>
        </li>
        <li>
          <p>
            If <m>\beta > 0</m>, <m>\alpha = 0</m> and
            <m>\delta \lt 0</m> then <m>(0,0)</m> is a centre.
          </p>
        </li>
      </ul>
    </p>
  </subsection>
</section>