<section xml:id="ordinary-points">
  <title>Ordinary Points</title>
  <subsection xml:id="subsection-ordinary-points-existence">
    <title>Existence of Solutions</title>
    <p>
      Consider a homogeneous linear second order differential
      equation.
      <me>
        y^{\prime \prime} + P(t) y^\prime + Q(t) y= 0
      </me>
      In a departure from the <xref ref="chapter-second-order-odes"
      />, I will now allow <m>P</m> and <m>Q</m> to be functions
      instead of just constants. Before I jump into the method of
      series solutions, I need some theory about the existence of
      solutions.
    </p>
    <definition>
      <statement>
        <p>
          A point <m>\alpha</m> is called an <term>ordinary
          point</term> for the differential equation if <m>P</m> and
          <m>Q</m> are both analytic at <m>\alpha</m>. Otherwise it
          is called a <term>singular point</term>. 
        </p>
      </statement>
    </definition>
    <theorem xml:id="thm-series-solutions-existence">
      <statement>
        <p>
          If <m>\alpha</m> is an ordinary point of a linear
          homogeneous second order differential equation, then there
          exists two linearly independent analytic solutions centered
          at <m>\alpha</m>. These analytic solutions will have radii
          of convergence at least as large as the distance from
          <m>\alpha</m> to the nearest singular point of the DE.
        </p>
      </statement>
    </theorem>
    <p>
      This is a lovley theorem, but these is one catch. The
      <sq>distance</sq> mentioned to the nearest singular point is
      actually distance in <m>\CC</m> to a possibly-complex singular
      point. In practice, this isn't too much of a worry, but I should
      be careful with my assumptions about the radii of convergence.
    </p>
  </subsection>
  <subsection xml:id="subsection-method-ordinary-points">
    <title>The Method for Solutions at Ordinary Points</title>
    <p>
      I could describe a general method, but it would be a lengthy and
      abstract description. Keeping everything very general, it would
      be easy to lose track of the pieces. Instead, I'll use examples
      to demonstrate the method. 
    </p>
    <example>
      <statement>
        <p>
          I'll start with a simple and known DE, to see how the
          method works.
          <me>
            y^{\prime \prime} + y = 0
          </me>
          Both <m>P</m> and <m>Q</m> are constant, so they analytic
          everywhere, even in <m>\CC</m>. Since there are no singular
          points, I expect solutions which have Taylor series defined
          for all of <m>\RR</m>. I can centre them at <m>0</m> for
          convenience. I assume the solution has a Taylor series.
          <me>
            y = \sum_{n=0}^\infty c_n t^n
          </me>
          I put this into the DE and calcluate, keeping in mind the
          tools to manipulate the inidices of series.
          <md>
            <mrow>
              y \amp = \sum_{n=0}^\infty c_n t^n
            </mrow>
            <mrow>
              y^\prime \amp = \sum_{n=1}^\infty c_n nt^{n-1}
            </mrow>
            <mrow>
              y^{\prime\prime} \amp = \sum_{n=2}^\infty c_n
              n(n-1)t^{n-2}
            </mrow>
            <mrow>
              y^{\prime \prime} + y \amp = \sum_{n=2}^\infty c_n
              n(n-1)t^{n-2} + \sum_{n=0}^\infty c_n t^n  = 0
            </mrow>
          </md>
          Now the DE has become an equation of infinite series. To
          solve this equation, I would like to express is as a single
          series. To do that, I usually will need to manipulate the
          indices. In this case, I shift the first series by 2 and
          then combine. 
          <md>
            <mrow>
              y^{\prime \prime} + y \amp = \sum_{n=0}^\infty
              c_{n+2}(n+2)(n+1)t^n + \sum_{n=0}^\infty c_n t^n = 0
            </mrow>
            <mrow>
              \amp = \sum_{n=0}^\infty \left[ c_{n+2}(n+2)(n+1) + c_n
              \right] t^n = 0
            </mrow>
          </md>
          Now I rewrite this last equation in a slightly different
          form.
          <me>
            \sum_{n=0}^\infty \left[ c_{n+2}(n+2)(n+1) + c_n \right]
            t^n = \sum_{n=0}^\infty 0 t^n
          </me>
          I've  just written the constant function <m>0</m> as a
          series. Now, two series are only equal is every coefficient
          is the same. Therefore, I can take this equation and turn
          it into equations of coefficients. There are infinitely many
          such equations (one for each natural number), but that's
          alright, since they have a pattern. For every <m>n \in
          \NN</m>, there is a recurrence relation.
          <me>
            (n+1)(n+2)c_{n+2} + c_n = 0 \implies c_{n+2} =
            \frac{-c_n}{(n+1)(n+2)}
          </me>
          To find the coefficients of the series that solves this DE,
          I have to solve this recurrence relation. I've essentially
          translated the problem: what was a differential equation
          problem is now a recurrence relation problem. I hope that
          solving the recurrence relation is easier than the original
          DE. There are various techniques in other parts of
          mathematics for solving recurrence relations. However, I am
          not assuming familiar with those techniques and, in this
          course, I will take a naive approach and try to solve them
          by inspection. 
        </p>
        <p>
          Before solving the recurrence relation, I need two starting
          terms, <m>c_0</m> and <m>c_1</m>. This works out very well,
          since <m>c_0 = y(0)</m> and <m>c_1 = y^\prime(0)</m>. The
          initial seed terms for the recurrence relation are exactly
          initial conditions for the DE. I can either leave them as
          variables <m>a</m> and <m>b</m>, or set them to specific
          values.
        </p>
        <p>
          Now I set <m>c_0 = 1</m> and <m>c_1 = 0</m>, which are the
          initial conditions given in the problem. (If I am not given
          initial conditions, I can leave these two as unknowns and
          carry them all they way through the process). Then I use
          the recurrence relation to calculate some terms. The general
          process of solving by inspection involves calcaulting the
          first few terms and trying to simply intuit a pattern in the
          term. 
          <md>
            <mrow>
              c_0 \amp = 1
            </mrow>
            <mrow>
              c_1 \amp = 0
            </mrow>
            <mrow>
              c_2 \amp = \frac{-c_0}{(1)(2)} = \frac{-1}{2}
            </mrow>
            <mrow>
              c_3 \amp = \frac{-c_1}{(2)(3)} = 0
            </mrow>
            <mrow>
              c_4 \amp = \frac{-c_2}{(3)(4)} = \frac{1}{2\cdot 3 \cdot
              4}
            </mrow>
            <mrow>
              c_5 \amp = \frac{-c_3}{(4)(5)} = 0
            </mrow>
            <mrow>
              c_6 \amp = \frac{-c_4}{(5)(6)} = \frac{-1}{2\cdot 3
              \cdot 4 \cdot 5 \cdot 6 }
            </mrow>
            <mrow>
              c_7 \amp = \frac{-c_5}{(6)(7)} = 0
            </mrow>
            <mrow>
              c_8 \amp = \frac{-c_6}{(7)(8)} = \frac{1}{8!}
            </mrow>
            <mrow>
              c_9 \amp = \frac{-c_7}{(8)(9)} = 0
            </mrow>
          </md>
          Having calculated a number of terms, a pattern is becoming
          clear. 
          <md>
            <mrow>
              c_{2n} \amp = \frac{(-1)^n}{(2n)!}
            </mrow>
            <mrow>
              c_{2n+1} \amp = 0
            </mrow>
          </md>
          Only the even terms are non zero. If a series has different
          behaviour between its even and its odd terms, I use this
          trick of writing <m>(2n)</m> to express the even terms and
          <m>(2n+1)</m> to express the odd terms. Since the odd terms
          vanish, I can write the resulting series only involving even
          term.
          <me>
            y = \sum_{n=0}^\infty \frac{(-1)^n}{(2n)!} t^{2n}
          </me>
          This is exactly the Taylor series for cosine, which makes
          perfect sense, since cosine solves the original DE and
          matches the initial conditions I imposed.
        </p>
      </statement>
    </example>
    <example>
      <statement>
        <p>
          This is the first example which has non-constant
          coefficients, since <m>Q = t</m>.
          <me>
            y^{\prime \prime} + ty = 0
          </me>
          <m>P=0</m> and <m>Q=t</m>, both of which are analytic
          everywhere, so I expect a series solution with infinite
          radius of convergence. I repeat the calculation from the
          previous example.
          <md>
            <mrow>
              y \amp = \sum_{n=0}^\infty c_n t^n
            </mrow>
            <mrow>
              y^\prime \amp = \sum_{n=1}^\infty c_n nt^{n-1}
            </mrow>
            <mrow>
              y^{\prime\prime} \amp = \sum_{n=2}^\infty c_n
              n(n-1)t^{n-2}
            </mrow>
            <mrow>
              y^{\prime \prime} + ty \amp = \sum_{n=2}^\infty c_n
              n(n-1)t^{n-2} + t\sum_{n=0}^\infty c_n t^n
            </mrow>
            <mrow>
              y^{\prime \prime} + ty \amp = \sum_{n=2}^\infty c_n
              n(n-1)t^{n-2} + \sum_{n=0}^\infty c_n t^{n+1}
            </mrow>
          </md>
          I've brought the <m>t</m> into the second series, which I
          have to do before I have any hope of combining them. Here, I
          could try to shift indices, but that wouldn't help yet since
          the exponent are different. I have to make the exponents
          match first. I'll shift both series so that the exponents
          are both <m>t^n</m>. This is shifting the index of the first
          series down by two and the index of the second series up by
          one.
          <md>
            <mrow>
              \amp = \sum_{n=2}^\infty c_{n+2} (n+2)(n+1) t^n +
              \sum_{n=1}^\infty c_{n-1} t^n
            </mrow>
          </md>
          Now the exponents are the same, but the starting indices are
          not. Shifting would mess up the exponents. So, instead, I
          take out terms. I'll take out the <m>0</m>th term from the
          first series so that they both start at 1. After that, I can
          finally combine the series. 
          <md>
            <mrow>
              \amp = 2c_2 + \sum_{n=1}^\infty c_{n+2} (n+2)(n+1) t^n +
              \sum_{n=1}^\infty c_{n-1} t^n
            </mrow>
          </md>
          <md>
            <mrow>
              \amp = 2c_2 + \sum_{n=1}^\infty \left[ c_{n+2}
              (n+2)(n+1) + c_{n-1} \right] t^n = 0
            </mrow>
          </md>
          Since the right side is zero, all these coefficients to be
          zero. The constnat coefficient on the left is just
          <m>2c_2=0</m>, which implies <m>c_2 = 0</m>. For the rest,
          <m>c_0</m> and <m>c_1</m> are unknown and I can use the
          series to generate a recurrence relation.
          <md>
            <mrow>
              (n+2)(n+1)c_{n+2} + c_{n-1} \amp = 0
            </mrow>
            <mrow>
              c_{n+2} \amp = \frac{-c_{n-1}}{(n+2)(n+1)}
            </mrow>
            <mrow>
              c_{n+3} \amp = \frac{-c_n}{(n+3)(n+2)}
            </mrow>
          </md>
          I shifted the recurrent relation in the last step, to make
          it a bit easier to read.  This is a third order recurrence
          relation, which might imply that three starting values are
          needed. However, there are still only two parameters. This
          isn't a problem, since I already calculated that
          <m>c_2=0</m>, which is essentially the third starting value.
          To try to see a pattern in the recurrence relation, I
          calculate some  coefficients.
          <md>
            <mrow>
              c_0 \amp = c_0
            </mrow>
            <mrow>
              c_1 \amp = c_1
            </mrow>
            <mrow>
              c_2 \amp = 0
            </mrow>
            <mrow>
              c_3 \amp = \frac{-c_0}{(3)(2)}
            </mrow>
            <mrow>
              c_4 \amp = \frac{-c_1}{(4)(3)}
            </mrow>
            <mrow>
              c_5 \amp = \frac{-c_2}{(5)(4)} = 0
            </mrow>
            <mrow>
              c_6 \amp = \frac{-c_3}{(6)(5)} =
              \frac{c_0}{(6)(5)(3)(2)}
            </mrow>
            <mrow>
              c_7 \amp = \frac{-c_4}{(7)(6)} =
              \frac{c_1}{(7)(6)(4)(3)}
            </mrow>
            <mrow>
              c_8 \amp = \frac{-c_5}{(8)(7)} = 0
            </mrow>
            <mrow>
              c_9 \amp = \frac{-c_6}{(9)(8)} =
              \frac{-c_0}{(9)(8)(6)(5)(3)(2)}
            </mrow>
            <mrow>
              c_{10} \amp = \frac{-c_7}{(10)(9)} =
              \frac{-c_1}{(10)(9)(7)(6)(4)(3)}
            </mrow>
            <mrow>
              c_{11} \amp = \frac{-c_8}{(11)(10)} = 0
            </mrow>
          </md>
          I see that there are three groups of terms. Like before,
          where I used an indexing trick to refer to even and odd
          terms, I can use a similar indexing trick to refer to these
          three groups of terms. 
        </p>
        <p><ul>
          <li>
            Terms of the form <m>c_{3n+2}</m> are all zero, since they
            all relate back to <m>c_2</m>.
          </li>
          <li>
            Terms of the form <m>c_{3n}</m> all involve <m>c_0</m>.
          </li>
          <li>
            Terms of the form <m>c_{3n+1}</m> all involve <m>c_1</m>.
          </li>
        </ul></p>
        <p>
          Expressing the coefficients in closed form is more difficult
          than before, but I still can intuite the general form. I
          use some factorial tricks to express the coefficients: the
          denominators are missing every third term, so if I mulitply
          numerator and denominator by those terms, I can write the
          denominator as a factorial. 
          <md>
            <mrow>
              c_{3n} \amp = \frac{(-1)^n (1)(4)(7)\ldots(3n-2)}{(3n)!}
              c_0
            </mrow>
            <mrow>
              c_{3n+1} \amp = \frac{(-1)^n
              (2)(5)(8)\ldots(3n-1)}{(3n+1)!} c_1
            </mrow>
            <mrow>
              c_{3n+2} \amp = 0
            </mrow>
          </md>
          Then I group the <m>c_1</m> terms into a series and the
          <m>c_2</m> terms into a series, to get a general solution.
          <md>
            <mrow>
              y = \amp c_0 \left[  1 + \sum_{n=n}^\infty \frac{(-1)^n
              (1)(4)(7)\ldots(3n-2)}{(3n)!} t^{3n} \right] + c_1
              \left[ t
            </mrow>
            <mrow>
              \amp + \sum_{n=0}^\infty \frac{(-1)^n
              (2)(5)(8)\ldots(n+2)}{(3n-1)!} t^{3n+1} \right]
            </mrow>
          </md>
          If I need to, I can easily check that each of these series
          has infinite radius of convergence.
        </p>
        <p>
          I might wonder: what are these functions? These are two
          new, strange and unfamiliar functions. Unless I have the
          good fortune (as in the previous example) to recognize the
          resulting Taylor series, I simply treat the solutions as
          new functions. However, I still consider the DE solved,
          since Taylor series can be used to define new functions. I
          can know a great  deal about a function based on its Taylor
          series, so this is a sufficient threshold of information to
          consider the DE solved.
        </p>
      </statement>
    </example>
    <example>
      <statement>
        <p>
          <md>
            <mrow>
              (t^2+1)y^{\prime \prime} + ty^\prime - y \amp = 0
            </mrow>
          </md>
          Before determining <m>P(t)</m> and <m>Q(t)</m>, I need to
          clear the coefficient of <m>y^{\prime \prime}</m>. This is
          important, since the definition of <m>P(t)</m> and
          <m>Q()t</m> (and hence the location of ordinary points)
          depends on the form where the coefficient of the second
          derivative is constant. 
          <md>
            <mrow>
              y^{\prime \prime} + \left( \frac{t}{t^2+1} \right)
              y^{\prime} - \left( \frac{1}{t^2+1} \right) y \amp = 0
            </mrow>
            <mrow>
              P(t) \amp = \frac{t}{t^2+1}
            </mrow>
            <mrow>
              Q(t) \amp = \frac{1}{t^2+1}
            </mrow>
          </md>
          <m>0</m> is an ordinary point, but what is the distance to
          the nearest singular point? Here, I need to remember to
          look for singularities in <m>\CC</m>. The denominators are
          undefined at <m>\pm \imath</m>, which is 1 unit away from
          the origin. Therefore, centered at <m>0</m>, I expect a
          radius of <m>R=1</m>.
        </p>
        <p>
          (As an aside, note that I can centre the series wherever we
          wish; I default to <m>0</m> simply because it is convenient
          and familiar. Each choice of a center point gives a
          different series solution, with a different radius of
          convergence. At <m>t=1</m>, I would have <m>R=
          \sqrt{2}</m> (the distance to <m>\imath</m> in <m>\CC</m>).
          At <m>t=4</m>, I would have <m>R = \sqrt{17}</m>.)
        </p>
        <p>
          This series solutions starts with a lengthly calculation.
          <md>
            <mrow>
              y \amp = \sum_{n=0}^\infty c_n t^n
            </mrow>
            <mrow>
              y^\prime \amp = \sum_{n=1}^\infty c_n nt^{n-1}
            </mrow>
            <mrow>
              y^{\prime\prime} \amp = \sum_{n=2}^\infty c_n
              n(n-1)t^{n-2}
            </mrow>
            <mrow>
              (t^2+1)y^{\prime \prime} + ty^\prime - y \amp = (t^2+1)
              \sum_{n=2}^\infty c_n n(n-1)t^{n-2} + t
              \sum_{n=1}^\infty c_n nt^{n-1} - \sum_{n=0}^\infty c_n
              t^n = 0 
            </mrow>
          </md>
          First, I need to distribute the <m>(t^2+1)</m>, which
          creates two series. At the same time, I take the powers of
          <m>t</m> into the series where they exists. 
          <md>
            <mrow>
              0 \amp = \sum_{n=2}^\infty n (n-1) c_n t^n +
              \sum_{n=2}^\infty n (n-1) c_n t^{n-2}
            </mrow>
            <mrow>
              \amp + \sum_{n=1}^\infty n c_n t^n -
              \sum_{n=0}^\infty c_n t^n
            </mrow>
          </md>
          Then I need to shift to make all the exponent <m>t^n</m>
          <md>
            <mrow>
              \amp = \sum_{n=2}^\infty n (n-1) c_n t^n +
              \sum_{n=0}^\infty (n+2) (n+1) c_{n+2} t^n
            </mrow>
            <mrow>
              \amp + \sum_{n=1}^\infty n c_n t^n -
              \sum_{n=0}^\infty c_n t^n
            </mrow>
          </md>
          The highest starting index is 2. Therefore, I'll pull out
          starting terms from any series that starts with an index
          below 2. 
          <md>
            <mrow>
              \amp = \sum_{n=2}^\infty n (n-1) c_n t^n + 2c_2 + 6c_3t
              + \sum_{n=2}^\infty (n+2) (n+1) c_{n+2} t^n
            </mrow>
            <mrow>
              \amp + c_1 t + \sum_{n=2}^\infty n c_n t^n
              - c_0 - c_1 t - \sum_{n=2}^\infty c_n t^n
            </mrow>
          </md>
          Finally, I can combine the four sums into one. I'll group
          all the other terms together as a constant and as a
          coefficient of <m>t</m>.
          <md>
            <mrow>
              \amp = (2c_2 - c_0) + (6c_3 + c_1 - c_1) t
            </mrow>
            <mrow>
              \amp + \sum_{n=2}^\infty \left[ n (n-1) c_n
              + (n+2) (n+1) c_{n+2} + n c_n - c_n \right] t^n = 0
            </mrow>
          </md>
          I proceed to find the recurrence relation by setting all
          the coefficients to <m>0</m>. I leave <m>c_0</m> and
          <m>c_1</m> as unknowns. I'll use some factoring and
          cancelling to make the recurrence relation more reasonable. 
          <md>
            <mrow>
              0 \amp = n (n-1) c_n + (n+2) (n+1) c_{n+2} + n c_n - c_n 
            </mrow>
            <mrow>
              (n+1) (n+2) c_{n+2} \amp = (1 - n - n(n-1)) c_n
            </mrow>
            <mrow>
              c_{n+2} \amp = \frac{-c_n (n^2-1)}{(n+2)(n+1)} =
              \frac{-c_n (n+1)(n-1)}{(n+2)(n+1)}
            </mrow>
            <mrow>
              \amp = \frac{ -c_n (n-1)}{n+2}
            </mrow>
          </md>
          This is a second order recurrence relation. Here are the
          first few terms. (I must be careful to use the isolated
          expressions to find <m>c_2</m> and <m>c_3</m>, and then the
          standard recurrence relation for <m>c_n</m> where <m>n \geq
          4</m>).
          <md>
            <mrow>
              c_0 \amp = c_0
            </mrow>
            <mrow>
              c_1 \amp = c_1
            </mrow>
            <mrow>
              c_2 \amp = \frac{c_0}{2}
            </mrow>
            <mrow>
              c_3 \amp = 0
            </mrow>
            <mrow>
              c_4 \amp = \frac{-c_2(1)}{4} = \frac{c_0}{(2)(4)}
            </mrow>
            <mrow>
              c_5 \amp = 0
            </mrow>
            <mrow>
              c_6 \amp = \frac{-c_4(3)}{6} =
              \frac{-c_0(3)}{(6)(4)(2)}
            </mrow>
            <mrow>
              c_7 \amp = 0
            </mrow>
            <mrow>
              c_8 \amp = \frac{-c_6(5)}{8} =
              \frac{c_0(5)(3)}{(8)(6)(4)(2)}
            </mrow>
            <mrow>
              c_9 \amp = 0
            </mrow>
            <mrow>
              c_{10} \amp = \frac{-c_8(7)}{10} =
              \frac{-c_0(7)(5)(3)}{(10)(8)(6)(4)(2)}
            </mrow>
            <mrow>
              c_{2n+1} \amp = 0
            </mrow>
            <mrow>
              c_{2n} \amp = \frac{(-1)^n (3)(5)(7)\ldots
              (2n-3)}{(2)(4)(6)(8) \ldots (2n)} c_0 = \frac{(-1)^n
              (2n-3)!}{(2)(4)(6) \ldots (2n-4) 2^n n!} c_0
            </mrow>
            <mrow>
              \amp = \frac{((-1)^n (2n-3)!}{2^{n-2} (n-2)! 2^n n!} c_0
              = \frac{((-1)^n (2n-3)!}{2^{2n-2} n! (n-2)!} c_0
            </mrow>
          </md>
          I have two cases. The odd terms all vanish, so the only
          place where I see <m>c_1</m> is the isolated term <m>c_1
          t</m>. That implies that the linear polynomial <m>c_1 t</m>
          is a solution for any <m>c_1</m>. For the <m>c_0</m> terms,
          there is still a whole series. Putting this together gives
          the general solution. Note that I have to start the series
          at <m>n=2</m>, since the pattern doesn't hold before that
          point.
          <me>
            y = c_0 \left[1 + \frac{t^2}{2} + \sum_{n=2}^\infty
            \frac{((-1)^n (2n-3)!}{2^{2n-2} n! (n-2)!} \right] + c_1
            t
          </me>
          If I look at the radius of convergence (due to the
          factorials in numerator and denominators) I can calculate
          the expected value of <m>R=1</m>. Note that the second
          term, the polynomial <m>c_1 t</m> doesn't have a domain
          restriction. It's possible to find solutions that exceed
          the limitation of the radius of convergence; <xref
          ref="thm-series-solutions-existence" /> guaranteed a
          solution with a minimum radius of convergence but did not
          stipulate a maximum.
        </p>
      </statement>
    </example>
  </subsection>
</section>
