<section xml:id="resonance">
  <title>Resonance</title>
  <introduction>
    <p>
      The discussion in the previous section about the similarity between forcing terms and the homogeneous solutions leads us into the subject of resonance in harmonic sequences.
      The question of resonance is this:
      is there a particular frequency for an external force on a harmonic system which produces the strongest effect?
    </p>
    <p>
      This is an important question in a number of situations.
      In music and acoustics, we may want to design explicitly for resonance.
      In the safety of structures,
      we would like to ensure that resonant behaviour is impossible.
    </p>
    <p>
      Let's start with the SOCCLDE describing an underdamped harmonic system. (Underdamped is necessary to allow for the possibility of resonance,
      as we will see in the calculations).
      Recall that for harmonic systems,
      the coefficients can be identified as mass <m>m</m>, spring constant <m>k</m>,
      coefficient of friction <m>b</m> and forcting <m>f(t)</m>.
      <me>
        m y^{\prime \prime} + b y^{\prime} + ky = f(t)
      </me>
    </p>
    <p>
      Look at the characterstic equation <m>mr^2 + br + k=0</m>.
      It has solutions
      <me>
        r = \frac{-b}{2m} \pm \frac{\sqrt{b^2-4km}}{2m}
      </me>.
    </p>
    <p>
      We can define a new constant to keep track of the behaviour.
      This constant is called the damping constant.
      <me>
        \zeta := \frac{b}{2\sqrt{km}}
      </me>
    </p>
    <p>
      The damping constant gives a nice measure of the friction.
      If <m>\zeta \lt  1</m> then the system is underdamped and we have sinusoidal behaviour.
      If <m>\zeta = 1</m> the situation is critically damped and if <m>\zeta > 1</m>,
      the situation is overdamped;
      in both cases, we just have exponential decay.
      The frictionless case is <m>\zeta = 0</m>.
      Let's go back to the frictionless case for a moment.
      The solutions when <m>\zeta = 0</m> are
      <me>
        y = A \cos \sqrt{\frac{k}{m}} t + B \sin \sqrt{\frac{k}{m}} t
      </me>.
    </p>
    <p>
      We're going to define another useful constant.
      <me>
        \omega := \sqrt{\frac{k}{m}}
      </me>
    </p>
    <p>
      This constant is called the natural frequency.
      It represents the frequency of sinusoidal oscillation in a perfect system without friction.
      (Note that all of the frequencies in this section are not true frequencies:
      they are off by a factor of <m>\frac{1}{2\pi}</m>.
      However, we'll ignore this fact and keep referring to them as frequencies.)
    </p>
    <p>
      Finally, we're going to define one more constant.
      <me>
        \lambda \defeq \frac{b}{2m}
      </me>
    </p>
    <p>
      If we look back to the underdamped case,
      the exponential decay term can be written <m>e^{-\lambda t}</m>.
      Therefore, <m>\lambda</m> is called the decay coefficient.
      With these new constants,
      the roots of the characteristic equation become
      <m>r = -\lambda +\pm \imath \sqrt{\omega^2 - \lambda^2}</m> and we can rewrite the homogeneous differential equation as
      <me>
        y^{\prime \prime} + 2\lambda y^\prime + \omega^2 y = 0
      </me>.
    </p>
    <p>
      Now let's return to the idea of a sinusoidal forcing term
      <m>f(t) = F\sin \gamma t</m> with some frequency <m>\gamma</m>.
      We want to look at four situation to understand the effect of this force and the possibility of resonance.
    </p>
  </introduction>
  <subsection xml:id="no-friction-no-forcing">
    <title>Situation 1: No Friction, No Forcing</title>
    <p>
      This is the trivial base case,
      where the system just oscillates forever with frequency <m>\omega</m>.
      This frequency is called the natural frequency because it describes the dynamics of this trivla base case,
      even if the ideal frictionless situation isn't particularly natural.
    </p>
  </subsection>
  <subsection xml:id="no-friction-forcing">
    <title>Situation 2: No Friction, Forcing</title>
    <p>
      The differential equation currently has the form
      <me>
        y^{\prime \prime} + \omega^2 y = F \sin \gamma t
      </me>.
    </p>
    <p>
      This is something that we can solve with undetermined coefficients.
      If we assume that <m>\gamma \neq \omega</m>,
      then the forcing term is unlike the homogeneous solutions.
      We use undetermined coefficients.
      <md>
        <mrow>y_p \amp  = C \sin \gamma t + D \cos \gamma C</mrow>
        <mrow>y_p^\prime \amp  = \gamma C \cos \gamma t - \gamma D \sin \gamma C</mrow>
        <mrow>y_p^{\prime \prime} \amp  = -\gamma^2 C \sin \gamma t - \gamma^2 D \cos \gamma C</mrow>
        <mrow>Ly_p \amp  = (-\gamma^2 C + \omega^2 C) \sin \gamma t + (-\gamma^2 D + \omega^2 D) \cos \gamma t = F \sin \gamma t</mrow>
        <mrow>-\gamma^2 C + \omega^2 C \amp  = F \implies C = \frac{F}{\omega^2 - \gamma^2 }</mrow>
        <mrow>-\gamma^2 D + \omega^2 D \amp  = 0 \implies D = 0</mrow>
        <mrow>y_p \amp  = \frac{F}{\omega^2 - \gamma^2} \sin \gamma t</mrow>
        <mrow>y \amp  = A \sin \omega t + B \cos \omega t + \frac{F}{\omega^2 - \gamma^2} \sin \gamma t</mrow>
      </md>
    </p>
    <p>
      We see that the particular solution is a sine wave with amplitutde <m>\frac{F}{\omega^2 - \gamma^2}</m>.
      The closer the forcing frequency is to the natural frequency,
      the greater the amplitude of the resulting oscillation.
      If we impose the initial conditions
      <m>y(0) = 0</m> and <m>y^\prime(0) = 0</m>,
      then the system is initially at rest and the only energy in the system comes from the external forcing.
      In this case,
      we easily get <m>B=0</m> from the first initial condition and we calculate for the second.
      <md>
        <mrow>y^{\prime} \amp  = \omega A \cos \omega t + \frac{\gamma F}{\omega^2 - \gamma^2} \cos \gamma t</mrow>
        <mrow>y^\prime (0) \amp  = A \omega + \frac{\gamma F}{\omega^2 - \gamma^2} = 0 \implies A = \frac{-\gamma F}{\omega(\omega^2 - \gamma^2)}</mrow>
        <mrow>y \amp  = \frac{-\gamma F}{\omega( \omega^2 - \gamma^2)} \sin \omega t + \frac{F}{\omega^2 - \gamma^2} \sin \gamma t = \frac{-\gamma F \sin \omega t + \omega F \sin \gamma t}{\omega (\omega^2 - \gamma^2)}</mrow>
      </md>
    </p>
    <p>
      Now, to answer the question of resonance,
      let's take the limit of this solution as <m>\gamma \rightarrow \omega</m>.
      The denominator is undefined,
      but the numerator also evaluates to <m>0</m>,
      so we can apply L'H&#xf4;pital's rule to calculate the limit.
      <md>
        <mrow>\lim_{\gamma \rightarrow \omega} \frac{-\gamma F \sin \omega t + \omega F \sin \gamma t}{\omega (\omega^2 - \gamma^2)} \amp  = \lim_{\gamma \rightarrow \omega} \frac{-F \sin \omega t + \omega t F \cos \gamma t}{-2\gamma \omega}</mrow>
        <mrow>\amp  = \frac{-F \sin \omega t + \omega t F \cos \omega t}{-2 \omega^2}</mrow>
        <mrow>\amp  = \frac{F}{2\omega^2} \sin \omega t - \frac{Ft \cos \omega t}{2\omega}</mrow>
      </md>
    </p>
    <p>
      The result has a <m>t \cos \omega t</m> term,
      which is a sinusoidal wave with linear growth in amplitude.
      The amplidute of the system will grow linearly without bound.
      This is the ideal (frictionless) understanding of resonance,
      where the oscillations of the system continue to grow.
    </p>
    <p>
      This is a justification, if you want,
      of why multiplying by <m>t</m> gives the particular solutions when you have a forcing term similar to the homogeneous solutions.
      When <m>\gamma = \omega</m>,
      the forcing is already a homogeneous solution,
      so expect a solution multiplied by <m>t</m>.
      That's precisely what we have here.
      It is also what we would have found if we with
      <m>\omega = \gamma</m> and used undetermined coefficients,
      instead of using the limit process.
    </p>
  </subsection>
  <subsection xml:id="friction-no-forcing">
    <title>Section 3: Friction, No Forcing</title>
    <p>
      The homogeneous SOCCLDE with our choice of constants is
      <me>
        y^{\prime \prime} + 2\lambda y^\prime + \omega^2 y = 0
      </me>.
    </p>
    <p>
      The characteristic equation is <m>r^2 + 2\lambda r + \omega^2</m> with roots
      <m>-\lambda \pm \imath \sqrt{\omega^2 - \lambda^2}</m> If we let <m>\omega_d = \sqrt{\omega^2 - \lambda^2}</m>,
      then the homogeneous solutions are
      <me>
        y= e^{-\lambda t} (A \cos \omega_d t + B \sin \omega_d t)
      </me>.
    </p>
    <p>
      The new constant <m>\omega_d</m> is called the damped frequency.
      It is not the same as the natural frequency,
      since friction changes the desire frequency of th system.
      We can observe from the previous definition that.
      <me>
        \lambda^2 = \frac{\zeta^2}{\omega^2} \hspace{2cm} \text{ or equivalently }  \hspace{2cm} \lambda^2 \omega^2 = \zeta^2
      </me>.
    </p>
    <p>
      Then we can also observe that
      <me>
        \omega_d = \omega \sqrt{1 - \zeta^2}
      </me>.
    </p>
    <p>
      With friction involved and no forcing,
      we have sinusoidally decaying oscillations where the frequency is this <m>\omega_d</m>.
      As an interesting aside,
      as <m>\zeta</m> approaches <m>1</m> and we approach the critical damped situation with simple exponential decay,
      this damped frequency approaches zero.
      This explains the transition from sinusoidal to exponential behaviour:
      as we approach the critically damped situation,
      the wavelength of the sine wave
      (which is a reciprocal of frequency)
      grows to <m>\infty</m>.
      The wave stretches out further and further until there isn't any wave left at all,
      just an exponential decay.
    </p>
  </subsection>
  <subsection xml:id="friction-forcing">
    <title>Situation 4: Friction and Forcing</title>
    <p>
      The differential equation is now
      <me>
        y^{\prime\prime} + 2\lambda y^\prime + \omega^2 y = F \sin \gamma t
      </me>.
    </p>
    <p>
      The homogeneous solutions are known from the third situation.
      <me>
        y_h = e^{-\lambda t} (A \cos \omega_d t + B \sin \omega_d t)
      </me>
    </p>
    <p>
      As in the second situation,
      our forcing term is <m>F\sin \gamma t</m> and has a particular frequency <m>\gamma</m>.
      Since the forcing lacks the exponential term,
      it is not the same as the homogeneous solutions.
      We can use undetermined coefficients without any alteration. (What does this already imply?) Here is the solution using undetermined coefficients,
      with some matrix algebra in the middle to solve the system of equations.
      <md>
        <mrow>\amp  \text{ Our Guess for Undetermined Coefficients: }</mrow>
        <mrow>y_p \amp  = C \sin \gamma t + D \cos \gamma t</mrow>
        <mrow>y_p^\prime \amp  = C \gamma \cos \gamma t - D \gamma \sin \gamma t</mrow>
        <mrow>y_p^{\prime \prime} \amp  = - C \gamma^2 \cos \gamma t - D \gamma^2 \sin \gamma t</mrow>
        <mrow>\amp  \text{ Solve for the Coefficients: }</mrow>
        <mrow>Ly_p \amp  = (-C\gamma^2 - 2\lambda D \gamma + C \omega^2) \sin \gamma t + (-D\gamma^2 + 2\lambda C \gamma + D \omega^2) \cos \gamma t</mrow>
        <mrow>-C\gamma^2 - 2\lambda D\gamma + C \omega^2 \amp  = F</mrow>
        <mrow>-D\gamma^2 + 2\lambda C\gamma + D \omega^2 \amp  = 0</mrow>
        <mrow>\left[ \begin{matrix} \omega^2 - \gamma^2 \amp  -2\lambda \gamma</mrow>
        <mrow>2\lambda \gamma \amp  \omega^2 - \gamma^2 \end{matrix} \right] \left[ \begin{matrix} C</mrow>
        <mrow>D \end{matrix} \right] \amp  = \left[ \begin{matrix} F</mrow>
        <mrow>0 \end{matrix} \right]</mrow>
        <mrow>M \amp  = \left[ \begin{matrix} \omega^2 - \gamma^2 \amp  -2\lambda \gamma</mrow>
        <mrow>2\lambda \gamma \amp  \omega^2 - \gamma^2 \end{matrix} \right]</mrow>
        <mrow>\det M \amp  = (\omega^2 - \gamma^2)^2 + 4 \lambda^2 \gamma^2</mrow>
        <mrow>M^{-1} \amp  = \frac{1}{ \det M} \left[ \begin{matrix} \omega^2 - \gamma^2 \amp  2 \lambda \gamma</mrow>
        <mrow>-2 \lambda \gamma \amp  \omega^2 - \gamma^2 \end{matrix} \right]</mrow>
        <mrow>\left[ \begin{matrix} C</mrow>
        <mrow>D \end{matrix} \right] \amp  = \frac{1}{\det M} \left[ \begin{matrix} \omega^2 - \gamma^2 \amp  2 \lambda \gamma</mrow>
        <mrow>-2 \lambda \gamma \amp  \omega^2 - \gamma^2 \end{matrix} \right] \left[ \begin{matrix} F</mrow>
        <mrow>0 \end{matrix} \right]</mrow>
        <mrow>C \amp  = \frac{(\omega^2 - \gamma^2) F}{(\omega^2 - \gamma^2)^2 + 4 \lambda^2 \gamma^2}</mrow>
        <mrow>D \amp  = \frac{-2\gamma\lambda F}{(\omega^2 - \gamma^2)^2 + 4 \lambda^2 \gamma^2}</mrow>
        <mrow>y_p \amp  = \frac{(\omega^2 - \gamma^2) F\sin \gamma t - 2 \gamma \lambda F \cos \gamma t}{(\omega^2 - \gamma^2)^2 + 4 \lambda^2 \gamma^2}</mrow>
        <mrow>y \amp  = e^{-\lambda t} (A \cos \omega_d t + B \sin \omega_d t) + \frac{(\omega^2 - \gamma^2) F\sin \gamma t - 2 \gamma \lambda F \cos \gamma t}{(\omega^2 - \gamma^2) + 4 \lambda^2 \gamma^2}</mrow>
      </md>
    </p>
    <p>
      As time passes,
      the homogeneous solutions fall out and only the term with the forcing frequency <m>\gamma</m> remains.
      What is its amplitude?
      The term is a linear combination of a sine and cosine wave,
      so we can use the identity mentioned previously that told us the amplitude of the combined wave was a pythagorean combination of the two amplitudes.
      <me>
        a = F \frac{\sqrt{(\omega^2 - \gamma^2)^2 + 4 \gamma^2 \lambda^2}}{(\omega^2 - \gamma^2)^2 + 4 \gamma^2 \lambda^2} = \frac{F}{\sqrt{(\omega^2 - \gamma^2)^2 + 4 \gamma^2 \lambda^2}}
      </me>
    </p>
    <p>
      The question of resonance now becomes a question of amplitude.
      If <m>F</m> is fixed,
      what is the maximum amplitude we can achieve with a fixed force?
      Note this amplitude is always finite <mdash/> with friction,
      there is no infinite growth of amplitude.
      (As predicted,
      since we didn't need to multiply by <m>t</m> when we setup the undetermined coefficients.)
      However, the amplitude can be quite large.
      This is a optimization problem,
      so we differentiate the expression for amplitude and find its critical points.
      <md>
        <mrow>a(\gamma) \amp  = \frac{F}{\sqrt{(\omega^2 - \gamma^2)^2 + 4 \gamma^2 \lambda^2}}</mrow>
        <mrow>a^\prime(\gamma) \amp  = \frac{-F(2 (\omega^2 - \gamma^2) (-2\gamma) + 8 \gamma \lambda^2)}{2((\omega^2 - \gamma^2)^2 + 4 \gamma^2 \lambda^2)^{\frac{3}{2}}} = 0</mrow>
        <mrow>4 \gamma (\omega^2 - \gamma^2) \amp = 8 \gamma \lambda^2</mrow>
        <mrow>\omega^2 - \gamma^2 \amp  = 2 \lambda^2</mrow>
        <mrow>\gamma^2 \amp  = \omega^2 - 2 \lambda^2</mrow>
        <mrow>\gamma \amp  = \sqrt{\omega^2 - 2 \lambda^2}</mrow>
      </md>
    </p>
    <p>
      This is almost in the form we want.
      Recall that <m>\lambda^2 = \omega^2 \zeta^2</m> which allows the form
      <me>
        \gamma = \sqrt{\omega^2 - 2 \zeta^2 \omega^2} = \omega \sqrt{1 - 2 \zeta^2}
      </me>.
    </p>
    <p>
      This is the critical point, and it is indeed a maximum for the amplitude.
      It is the resonant frequency.
      However, are we certain that it exists?
      We need <m>1-2\zeta^2</m> to be positive to define this square root.
      This implies, certainly, that <m>\zeta \lt  1</m>,
      which we assumed when we decided to work with the underdamped case
      (that assumption is now justified).
      However, the inequality is stricter.
      <me>
        \zeta^2 \leq \frac{1}{2} \implies \zeta \leq \frac{1}{\sqrt{2}}
      </me>
    </p>
    <p>
      The bound for the damping coefficient is smaller than simply for the underdamped case.
      The conclusion we reach is that a resonant frequency only exists is the friction is minimal enough,
      measured by this <m>\zeta \lt \frac{1}{\sqrt{2}}</m>.
      In particular,
      if we are concerned about safety and want to avoid the situation of resonant frequency,
      we know how much friction we need to build into the system.
    </p>
  </subsection>
</section>