<section xml:id="section-variation-parameters">
  <title>Variation of Parameters</title>
  <introduction>
    <p>
      Undetermined coefficients is an effective and efficient
      (relatively speaking!) way to solve for a particular
      non-homogeneous solution of a SOLCCDE. It's restriction is its
      scope: it only works for specific forcing terms.  Variation of
      parameters is a much more general method of finding particular
      solutions.  It's weakness is the reliance on difficult integrals
      <mdash/> often we'll have to leave the solutions in a form which
      involves unfinished integrals.  In the examples, we'll often
      stick to forcing terms which could have used undetermined
      coefficients, just to make the integrals reasonable.
    </p>
  </introduction>
  <subsection xml:id="subsection-wronskians">
    <title>Wronskians</title>
    <definition>
      <statement>
        <p>
          Let <m>f_1, f_2, \ldots f_n \in C^{n-1}(\RR)</m>.  The
          <term>Wronskian</term> of this set of functions is defined
          to be the determinant of a matrix involving the <m>f_i</m>
          and their derivatives.
          <me>
            W(f_1, f_2, \ldots, f_n) : = \left| \begin{matrix} f_1
            \amp \ldots \amp f_n \\ f^\prime_1 \amp \ldots \amp
            f^\prime_n \\ f^{\prime\prime}_1 \amp \ldots \amp
            f^{\prime\prime}_n \\ \ldots \amp \ldots \amp \ldots \\
            f^{(n-1)}_1 \amp \ldots \amp f^{(n-1)}_n \end{matrix}
            \right|
          </me>
        </p>
      </statement>
    </definition>
    <p>
      The Wronskian of a set of functions has a number of different
      uses.  Its first use is checking for linear independence.  The
      set of functions linearly independent if and only if the
      Wronskian is never zero.  Most of the time, this is easy to
      satisfy.  In addition, if we have linearly independent
      functions, we know the Wronskian is never zero and we can divide
      by if with impunity.
    </p>
    <p>
      For variation of parameters, we only need to the Wronskain of
      two functions.  The definition here is relatively simple.
      <me>
        W(f_1,f_2) = \left| \begin{matrix} f_1 \amp f_2 \\ f_1^\prime
        \amp f_2^\prime \end{matrix} \right| = f_1 f_2^\prime - f_2
        f_1^\prime
      </me>
    </p>
  </subsection>
  <subsection xml:id="subsection-technique-vop">
    <title>The Technique of Variations of Parameters</title>
    <p>
      Let <m>L</m> be the second order operator
      <me>
        L = \frac{d^2}{dt^2} +P \frac{d}{dt} + Q
      </me>.
      Let <m>y_1</m> and <m>y_2</m> be solutions to the homogeneous
      equation <m>Ly=0</m>.  The general solution to the homogeneous
      equation is <m>Ay_1 + By_2</m>.  As with the first-order case,
      variation of parameters replaces the constants <m>A</m> and
      <m>B</m> with functions.  That is, we look for a solution which
      has the form (where <m>u_1(t)</m> and <m>u_2(t)</m> are unknown
      functions)
      <me>
        y_p = u_1 y_1 + u_2 y_2
      </me>.
      Then we put this <m>y_p</m> into the differential equation.
      A long and tedious calculation ensues.
      <md>
        <mrow>
          Ly_p \amp = u_1^{\prime \prime} y_1 + 2 u_1^\prime
          y_1^\prime + u_1 y_1^{\prime \prime} + u_2^{\prime \prime}
          y_2 + 2 u_2^\prime y_2^\prime + u_2 y_2^{\prime \prime} + P
          \left( u_1^\prime y_1 + u_1 y_1^\prime + u_2^\prime y_2 +
          u_2 y_2^\prime \right)
        </mrow>
        <mrow>
          \amp Q \left( u_1 y_1 + u_2 y_2 \right) = f
        </mrow>
        <mrow>
          \amp = u_1 \left( y_1^{\prime \prime} + Py_1^\prime + Q y_1
          \right) + u_2 \left( y_2^{\prime \prime} + Py_2^\prime + Q
          y_2 \right) + (y_1 u_1^{\prime \prime} + u_1^\prime
          y_1^\prime) + (y_2 u_2^{\prime \prime} + u_2^\prime
          y_2^\prime)
        </mrow>
        <mrow>
          \amp + P \left( y_1 u_1^\prime + y_2 u_2^\prime \right) +
          y_1^\prime u_1^\prime + y_2^\prime u_2^\prime = f
        </mrow>
        <mrow>
          \amp = u_1 (L y_1) + u_2 (L y_2) + \frac{d}{dt} \left( y_1
          u_1^\prime \right) + \frac{d}{dt} \left( y_2 u_2^\prime
          \right) + P \left( y_1 u_1^\prime + y_2 u_2^\prime \right) +
          \left( y_1^\prime u_1^\prime + y_2^\prime u_2^\prime \right)
          = f
        </mrow>
        <mrow>
          \amp = 0 + 0 + \frac{d}{dt} \left(y_1 u_1^\prime + y_2
          u_2^\prime \right) + P \left( y_1 u_1^\prime + y_2
          u_2^\prime \right) + \left( y_1^\prime u_1^\prime +
          y_2^\prime u_2^\prime \right) = f
        </mrow>
      </md>
      So far, this doesn't look particularly useful.  Part of the
      problem is that we've given ourselves too much freedom.
      Choosing two entirely unknown functions is not limiting enough.
      The advantage of this situation is that we can impose a
      reasonable restriction while still allowing for general
      solutions.  We impose the restriction <m>y_1 u_1^\prime + y_2
      u_2^\prime = 0</m>.  (Why this restriction?  Because it works,
      and somewhere in matheamtical history, some clever mathematician
      figured out that it works.) This restriction removes two terms
      from the previous equation and leaves us with a simple
      equation.
      <me>
        \left( y_1^\prime u_1^\prime + y_2^\prime u_2^\prime \right) =
        f
      </me>
      If we remember the restriction, we now have a system of two
      equations.
      <md>
        <mrow>
          y_1 u_1^\prime + y_2 u_2^\prime \amp = 0
        </mrow>
        <mrow>
          y_1^\prime u_1^\prime + y_2^\prime u_2^\prime \amp = f
        </mrow>
      </md>
      We can express this system in matrix terminology.
      <me>
        \begin{pmatrix}0\\f\end{pmatrix} = \left( \begin{matrix} y_1
        \amp y_2 \\ y_1^\prime \amp y_2^\prime \end{matrix} \right)
        \begin{pmatrix}u_1^\prime\\u_2^\prime\end{pmatrix}
      </me>
      Linear algebra then solves the system.  Conveniently, the
      determinant of the system is the Wronskian <m>W(y_1,y_2)</m>,
      which we will simply write <m>W</m> for the remainder of this
      derivation.
      <md>
        <mrow>
          u_1^\prime \amp = \frac{-y_2 f}{W}
        </mrow>
        <mrow>
          u_2^\prime \amp = \frac{y_1 f}{W}
        </mrow>
      </md>
      The solution gives us the derivatives of <m>u_1</m> and
      <m>u_2</m>, so we can integrate.
      <md>
        <mrow>
          u_1 \amp = - \int \frac{y_2 f}{W} dt
        </mrow>
        <mrow>
          u_2 \amp = \int \frac{y_1 f}{W} dt
        </mrow>
      </md>
      We insert these <m>u_i</m> in the original expression.
      <me>
        y_p = \left( -\int \frac{y_2 f}{W} dt \right) y_1 + \left(
        \int \frac{y_1 f}{W} dt \right) y_2
      </me>
      Therefore, the general solution to the original equation <m>Ly =
      f</m> is 
      <me>
        y_p = \left( -\int \frac{y_2 f}{W} dx \right) y_1 + \left(
        \int \frac{y_1 f}{W} dt \right) y_2 + Ay_1 + By_2
      </me>.
      Note that this general form implies, conveniently, that we don't
      have to worry about constants of integration in either of the
      two integrals.  If we had a constant of integration, it would
      lead to a multiple of one of the homogeneous solutions.  Those
      multiples are already accounted for in the general homogeneous
      solution.
    </p>
    <example>
      <statement>
        <p>
          This example is from Roberts and Marion.
          <md>
            <mrow>
              y^{\prime\prime} - 2y^{\prime} + 2y \amp = 2e^t
            </mrow>
            <mrow>
              r^2 -2r +2 \amp = 0
            </mrow>
            <mrow>
              r \amp = 1 \pm \imath
            </mrow>
            <mrow>
              y_1 \amp = e^t \cos t
            </mrow>
            <mrow>
              y_2 \amp = e^t \sin t
            </mrow>
            <mrow>
              y_1^\prime \amp = e^t \cos t - e^t \sin t
            </mrow>
            <mrow>
              y_2^\prime \amp = e^t \sin t + e^t \cos t
            </mrow>
            <mrow>
              W \amp = e^t \cos t (e^t \sin t + e^t \cos t) - e^t \sin
              t (e^t \cos t - e^t \sin t)
            </mrow>
            <mrow>
              \amp = e^{2t} (\cos t \sin t + \cos^2 t - \sin t \cos t
              + \sin^2 t) = e^{2t}
            </mrow>
            <mrow>
              u_1 \amp = \int \frac{-y_2 f}{W} dt = -\int \frac{ e^t
              \sin t 2e^t}{e^{2t}}dt
            </mrow>
            <mrow>
              \amp = -2 \int \sin t dt = 2 \cos t
            </mrow>
            <mrow>
              u_2 \amp = \int \frac{y_1 f}{W} dt = \int \frac{ e^t
              \cos t 2e^t}{e^{2t}}dt
            </mrow>
            <mrow>
              \amp = 2 \int \cos t dt = 2 \sin t
            </mrow>
            <mrow>
              y_p \amp = 2\cos t e^t \cos t + 2 \sin t e^t \sin t =
              2e^t
            </mrow>
            <mrow>
              y \amp = 2e^t + Ae^t \cos t + B e^t \sin t
            </mrow>
          </md>
        </p>
      </statement>
    </example>
    <example>
      <statement>
        <p>
          <md>
            <mrow>
              y^{\prime\prime} - 4y^{\prime} + 4y \amp = (t+1)e^{2t}
            </mrow>
            <mrow>
              r^2 -4r +4 \amp = 0
            </mrow>
            <mrow>
              r \amp = 2
            </mrow>
            <mrow>
              y_1 \mp = e^{2t}
            </mrow>
            <mrow>
              y_2 \amp = te^{2t}
            </mrow>
            <mrow>
              y_1^\prime \amp = 2e^{2t}
            </mrow>
            <mrow>
              y_2^\prime \amp = 2te^{2t} + e^{2t}
            </mrow>
            <mrow>
              W \amp = e^{2t} (e^{2t} + 2te^{2t}) - te^{2t} 2e^{2t} =
              e^{4t}
            </mrow>
            <mrow>
              u_1 \amp = \int \frac{-y_2 f}{W} dt = -\int
              \frac{te^{2t}(t+1)e^{2t}}{e^{4t}} dt
            </mrow>
            <mrow>
              \amp = - \int t^2 + t = \frac{-t^3}{3} - \frac{t^2}{2}
            </mrow>
            <mrow>
              u_2 \amp = \int \frac{y_1 f}{W} dt = \int \frac{ e^{2t}
              (t+1)e^{2t}}{e^{4t}} dt
            </mrow>
            <mrow>
              \amp = \int t+1 dt = \frac{t^2}{2} + t
            </mrow>
            <mrow>
              y_p \amp = \left( \frac{-t^3}{3} - \frac{t^2}{2} \right)
              e^{2t} + \left( \frac{t^2}{2} + t \right) te^{2t}
            </mrow>
            <mrow>
              \amp = \frac{t^3 e^{2t}}{6} + \frac{t^2e^2t}{2}
            </mrow>
            <mrow>
              y \amp = \frac{t^3 e^{2t}}{6} + \frac{t^2e^2t}{2} +
              Ae^{2t} + Bte^{2t}
            </mrow>
          </md>
        </p>
      </statement>
    </example>
    <example>
      <statement>
        <p>
          This is (finally) an example that couldn't have used
          undetermined coefficients.
          <md>
            <mrow>
              y^{\prime\prime} + 9y \amp = \csc 3t
            </mrow>
            <mrow>
              r^2 + 9 \amp = 0
            </mrow>
            <mrow>
              r \amp = \pm 3\imath
            </mrow>
            <mrow>
              y_1 \amp = \cos 3t
            </mrow>
            <mrow>
              y_2 \amp = \sin 3t
            </mrow>
            <mrow>
              y_1^\prime \amp = -3 \sin 3t
            </mrow>
            <mrow>
              y_2^\prime \amp = 3 \cos 3t
            </mrow>
            <mrow>
              W \amp = 3\cos^2 3t + 3 \sin^2 3t = 3
            </mrow>
            <mrow>
              u_1 \amp = \int \frac{-y_2 f}{W} dt = -\int \frac{\sin
              3t \csc 3t}{3} dt = \frac{-1}{3} \int dt = \frac{-t}{3}
            </mrow>
            <mrow>
              u_2 \amp = \int \frac{y_1 f}{W} dt = \int \frac{\cos3t
              \csc 3t}{3} dt = \frac{1}{3} \int \cot 3t = \frac{1}{9}
              \ln |\sin 3t|
            </mrow>
            <mrow>
              y_p \amp = \frac{-t}{3} \cos 3t + \frac{\sin 3t \ln
              |\sin 3t|}{9}
            </mrow>
            <mrow>
              y \amp = \frac{-t}{3} \cos 3t + \frac{\sin 3t \ln |\sin
              3t|}{9} + A \cos 3t + B \sin 3t
            </mrow>
          </md>
          One of the reasons that undetermined coefficients wouldn't
          have worked is that the form of the particular solution,
          <m>\ln |\sin 3t|</m>, is not a function likely to be
          guessed.
        </p>
      </statement>
    </example>
    <example>
      <statement>
        <p>
          In this example, the resulting integrals are not expressable
          by elementary functions.  In these cases, we just leave the
          integrals in the final solution.  We just have to live with
          these unexpressible function (or, I suppose, come up with
          new names for them.)
          <md>
            <mrow>
              y^{\prime\prime} - y \amp = \frac{1}{t}
            </mrow>
            <mrow>
              r^2 - 1 \amp = 0
            </mrow>
            <mrow>
              r \amp = \pm 1
            </mrow>
            <mrow>
              y_1 \amp = e^t
            </mrow>
            <mrow>
              y_2 \amp = e^{-t}
            </mrow>
            <mrow>
              y_1^\prime \amp = e^t
            </mrow>
            <mrow>
              y_2^\prime \amp = - e^{-t}
            </mrow>
            <mrow>
              W \amp = -1 -1 = -2
            </mrow>
            <mrow>
              u_1 \amp = \int \frac{-y_2 f}{W} dt = -\int \frac{
              e^{-t} \frac{1}{t}}{-2} = \frac{1}{2} \int
              \frac{e^{-t}}{t} dt
            </mrow>
            <mrow>
              u_2 \  =nt \frac{y_1 f}{W} dt = \int \frac{ e^t
              \frac{1}{t}}{-2} = \frac{-1}{2} \int \frac{e^t}{t} dt
            </mrow>
            <mrow>
              y_p \amp \frac{e^t}{2} \int \frac{e^{-t}}{t} dt -
              \frac{e^{-t}}{2} \int \frac{e^t}{t} dt
            </mrow>
            <mrow>
              y \amp \frac{e^t}{2} \int \frac{e^{-t}}{t} dt -
              \frac{e^{-t}}{2} \int \frac{e^t}{t} dt + Ae^t + Be^{-t}
            </mrow>
          </md>
        </p>
      </statement>
    </example>
  </subsection>
</section>
