<section xml:id="substitutions">
  <title>Substitutions</title>
  <introduction>
    <p>
      The third and final technique we will study for first order DEs is substitution.
      At some level,
      solving DEs is a more complicated and involved version of doing integrals,
      since we are trying to undo the results of differentiation.
      Substitution is the most common and important technique for solving integrals.
      It takes complicated integrals and changes their setup to make them more approachable.
      The technique is exactly the same here:
      we change the DE with some substitution operation to turn it into something we already know how to do.
      As with substitution for integrals,
      we can recognize some typical forms,
      but many others require creativity and ingenuity to solve.
      In this section, we'll introduce two forms which use substitution.
    </p>
  </introduction>
  <subsection xml:id="homogeneous">
    <title>Homogeneous DEs</title>
    <p>
      The first substitution is for a class of terribly named DEs called homogenous equations.
      Please note, this homogeneous has <em>nothing</em>
      to do with the previous definition for linear equations.
      The word here comes from a different use of the term in algebra.
      In any case, a homogenous DE has the form
      <me>
        \frac{dy}{dt} = f \left( \frac{y}{t} \right)
      </me>.
    </p>
    <p>
      The substitution is the relatively obvious replacement <m>v = \frac{y}{t}</m>.
      The right side of the equation easily turns into <m>f(v)</m>,
      but the transformation of the left side is trickier.
      <md>
        <mrow>y \amp  = tv</mrow>
        <mrow>f(v) = \frac{dy}{dt} \amp  = v + t \frac{dv}{dt}</mrow>
        <mrow>\frac{dv}{dt} \amp  = \frac{f(v) - v}{t}</mrow>
        <mrow>\int \frac{dv}{f(v)-v} \amp  = \int \frac{dt}{t}</mrow>
      </md>
    </p>
    <p>
      In the last step,
      we've already started to solve the homogeneous equation as a seperable equation after the substitution is complete.
    </p>
    <example>
      <statement>
        <p>
          This example is from Roberts and Marion.
          It is technically a seperable equation,
          but it is still useful to see how the substitution technique works.
          <md>
            <mrow>\frac{dy}{dt} \amp  = \frac{t}{y}</mrow>
            <mrow>v \amp  =\frac{y}{t}</mrow>
            <mrow>f(v) \amp  = \frac{1}{v}</mrow>
            <mrow>\frac{dv}{dt} \amp  = \frac{\frac{1}{v} - v}{t}</mrow>
            <mrow>\int \frac{dv}{\frac{1}{v} -v} \amp  = \int \frac{dt}{t}</mrow>
            <mrow>\int \frac{v}{1-v^2} dv \amp  = \ln |t| + c</mrow>
            <mrow>\frac{-1}{2} \ln |1-v^2| \amp  = \ln |t| + C</mrow>
            <mrow>\frac{1}{\sqrt{1-v^2}} \amp  = ct</mrow>
            <mrow>\sqrt{1-v^2} \amp  = \frac{c}{t}</mrow>
            <mrow>1-v^2 \amp  = \frac{c}{t^2}</mrow>
            <mrow>v^2 \amp  = 1 - \frac{c}{t^2}</mrow>
            <mrow>v \amp  = \pm \sqrt{ 1 - \frac{c}{t^2}}</mrow>
            <mrow>\frac{y}{t} \amp  = \pm \sqrt{ 1 - \frac{c}{t^2}}</mrow>
            <mrow>y \amp  = \pm t \sqrt{1 - \frac{c}{t^2}} = \pm \sqrt{t^2 - c}</mrow>
          </md>
        </p>
        <p>
          Notice that we reverse the substitution at the end,
          so that we end with the same variables as we started with.
        </p>
      </statement>
    </example>
    <example>
      <statement>
        <md>
          <mrow>\frac{dy}{dt} \amp  = \frac{-y^2 - yt }{t^2} = \frac{-y^2}{t^2} -
          \frac{y}{t}</mrow>
          <mrow>v \amp  = \frac{y}{t}</mrow>
          <mrow>f(v) \amp  = -v^2 -v</mrow>
          <mrow>\frac{dv}{dt} \amp  = \frac{f(v) - v}{t} = \frac{-v^2 -v -v}{t} =
          \frac{-v^2 - 2v}{t}</mrow>
          <mrow>\int \frac{dv}{-v^2-2v} \amp  = \int \frac{dt}{t} = \ln |t| + c</mrow>
          <mrow>\frac{1}{-v^2 - 2v} \amp  = \frac{-1}{v(2+v)} = \frac{1}{2}
          \frac{1}{v+2} + \frac{-1}{2} \frac{1}{v} \hspace{1cm}
          \text{ (Partial Fractions) }</mrow>
          <mrow>\frac{1}{2} \int \frac{dv}{v+2} + \frac{-1}{2} \int \frac{dv}{v}
          \amp  = \ln |t| + c</mrow>
          <mrow>\frac{1}{2} \ln |v+2| + \frac{-1}{2} \ln |v| \amp  = \ln |t| + c</mrow>
          <mrow>\ln |v+2|^{\frac{1}{2}} + \ln |v|^\frac{-1}{2} \amp  = \ln |t| + c</mrow>
          <mrow>\sqrt{1 + \frac{2}{v}} \amp  = ct</mrow>
          <mrow>\frac{1 + \sqrt{2}}{v} \amp  = ct</mrow>
          <mrow>1 + \frac{2}{v} \amp  = ct^2</mrow>
          <mrow>\frac{2}{v} \amp  = ct^2 -1</mrow>
          <mrow>v \amp  = \frac{2}{ct^2 -1}</mrow>
          <mrow>\frac{y}{t} \amp  = \frac{2}{ct^2 - 1}</mrow>
          <mrow>y \amp  = \frac{2t}{ct^2 -1}</mrow>
        </md>
      </statement>
    </example>
  </subsection>
  <subsection xml:id="bernoulli">
    <title>Bernoulli Equations</title>
    <p>
      The other substitution is for a class of DEs called Bernoulli equations.
    </p>
    <p>
      These equations are almost linear,
      but they have an extra <m>y^n</m> term.
      The most general form is
      <me>
        \frac{dy}{dt} + P(t) y = Q(t) y^n
      </me>.
    </p>
    <p>
      The substitution is <m>v = y^{1-n}</m>.
      Be careful: this is <m>y^{1-n}</m>, not <m>y^{n-1}</m>.
      It's a very easy mistake to get this exponent wrong.
      We transform the DE by looking at the following derivations.
      <md>
        <mrow>\frac{dv}{dt} \amp  = (1-n) y^{1-n-1} \frac{dy}{dt} = (1-n)y^{-n} \frac{dy}{dt}</mrow>
        <mrow>\amp  = (1-n)y^{-n} \left( Q(t) y^n - P(t) y \right) = (1-n) Q(t) - (1-n) P(t) y^{1-n}</mrow>
        <mrow>\amp = (1-n) Q(t) - (1-n) P(t) v</mrow>
        <mrow>\frac{dv}{dt} + (1-n)v P(t) \amp  = (1-n) Q(t)</mrow>
      </md>
    </p>
    <p>
      This is now a linear equation in <m>v</m>.
      We can solve it as a linear equation in <m>v</m> and then use the reverse substitution to get back to <m>y</m>.
    </p>
    <example>
      <statement>
        <p>
          This example is from Roberts and Marion.
          <md>
            <mrow>\frac{dy}{dt} - \frac{1}{2} \frac{y}{t} \amp  = -e^t y^3</mrow>
            <mrow>n \amp  =3</mrow>
            <mrow>v \amp  = y^{-2}</mrow>
            <mrow>\frac{dv}{dt} - (-2) v \frac{1}{2t} \amp  = -2 (-e^t) = 2e^t</mrow>
            <mrow>\frac{dv}{dt} + \frac{v}{t} \amp  = 2e^t</mrow>
          </md>
        </p>
        <p>
          This is a familiar linear equation which was solved in <xref ref="linear-example1">Example</xref>.
          We recall the solution from before.
          <md>
            <mrow>v \amp  = 2e^t \left( 1 + \frac{1}{t} \right) + \frac{c}{t}</mrow>
            <mrow>y^{-2} \amp  = 2e^t \left( 1 + \frac{1}{t} \right) + \frac{c}{t}</mrow>
            <mrow>y \amp  = \left( 2e^t \left( 1 + \frac{1}{t} \right) + \frac{c}{t} \right)^{\frac{-1}{2}}</mrow>
            <mrow>y \amp  = \frac{\pm1}{\sqrt{2e^t \left( 1 + \frac{1}{t} \right) + \frac{c}{t}}}</mrow>
          </md>
        </p>
      </statement>
    </example>
    <example>
      <statement>
        <md>
          <mrow>\frac{dy}{dt} \amp  = y(ty^3 -1) = ty^4 - y</mrow>
          <mrow>\frac{dy}{dt} + y \amp  = ty^4</mrow>
          <mrow>v \amp  = y^{-3}</mrow>
          <mrow>\frac{dv}{dt} - 3v \amp  = -3t</mrow>
          <mrow>P(t) \amp  = -3</mrow>
          <mrow>Q(t) \amp  = -3t</mrow>
          <mrow>\mu(t) \amp  = e^{\int P(t) dt} = e^{-3t}</mrow>
          <mrow>\frac{d}{dt} e^{-3t} v \amp  = -3t e^{-3t}</mrow>
          <mrow>e^{-3t} v \amp  = \int -3t e^{-3t} dt = -3 \left(
          \frac{te^{-3t}}{-3} - \int \frac{e^{-3t}{-3}} dt \right)</mrow>
          <mrow>e^{-3t} v \amp  = t e^{-3t} - \int e^{-3t} dt = t e^{-3t} +
          \frac{e^{-3t}}{3} + c</mrow>
          <mrow>v = \amp  t + \frac{1}{3} + ce^{3t} = \frac{3t + 1 + ce^{3t}}{3}</mrow>
          <mrow>y^{-3} \amp  = \frac{3t + 1 + ce^{3t}}{3}</mrow>
          <mrow>y^3 \amp  = \frac{3}{3t + 1 + ce^{3t}}</mrow>
          <mrow>y \amp  = \sqrt[3]{\frac{3}{3t + 1 + ce^{3t}}}</mrow>
        </md>
      </statement>
    </example>
  </subsection>
</section>