<section xml:id="undetermined-coefficients">
  <title>The Method of Undetermined Coefficients</title>
  <p>
    Undetermined coefficients is the first of two methods we use to solve non-homogeneous SOCCLDEs.
    The second method, variation of parameters, is more general,
    but undetermined coefficients is easier and faster for particular types of non-homogemeous terms.
    In the spirit of applications to harmonic motion, I will often refer to the non-homogenous part of the SOCCLDE as a forcing term.
  </p>
  <p>
    Recall, before we start,
    that if <m>Ly = f(t)</m> is a non-homogeneous SOCCLDE, we know the structure of the general family of solutions.
    We expect two linearly independent solutions,
    <m>y_1</m> and <m>y_2</m>, for the homogenous equaiton <m>Ly = 0</m>.
    We look for only one particular solution <m>y_p</m> of <m>Ly = f(t)</m>.
    The general solution has the form (where <m>\alpha</m> and <m>\beta</m> are real parameter)
    <me>
      y = y_p + \alpha y_1 + \beta y_2
    </me>.
  </p>
  <p>
    Undetermined coefficents and variation of parameters try to find this particular solution <m>y_p</m>,
    and then we use the homogenous solutions to write the complete family.
  </p>
  <p>
    The idea of undetermined coefficients is relatively simple:
    we try to guess a particular solution which is the same type of function as the forcing.
    If the forcing is polynomial,
    we look for a polynomial solution;
    if the forcing is exponential,
    we look for an exponential solution;
    and if the foring is sinusoidal,
    we look for a sinusoidal solution.
    Undertermined coefficients is going to work well for these three types of forcing terms or forcing terms given by products of functions of these types.
    However, it doesn't apply to other types of functions,
    where we can't reasonably expect the solution to look like the forcing term.
  </p>
  <p>
    There is one possible pitfall to the process:
    sometimes the forcing terms is similar to the homogeneous solutions.
    In this case,
    the same type of function will only solve the homogeneous equation,
    not the non-homogeneous case.
    Our solution here is reminiscent of the case of repeated roots:
    we multiply by the independent variable <m>t</m> until we get something new.
    We'll see how this works out in examples.
  </p>
  <p>
    Before we get into examples, here is a useful chart.
    As I said, we want to guess a similar type of functions to the forcing.
    What is similar?
    This chart gives the guesses.
    The constants <m>C_i</m> and <m>D_j</m> need to be determined:
    these constants are the undetermined coefficients which give the process its name.
  </p>
  <tabular>
    <row>
      <cell><m>f(t)</m></cell>
      <cell><m>y_p</m></cell>
    </row>
    <row bottom="minor">
      <cell></cell>
      <cell></cell>
    </row>
    <row>
      <cell><m>ke^{at}</m></cell>
      <cell><m>Ce^{at}</m></cell>
    </row>
    <row>
      <cell><m>kt^n</m></cell>
      <cell><m>C_n t^n + C_{n-1}t^{n-1} + \dots + C_1 t + C_0</m></cell>
    </row>
    <row>
      <cell><m>k \cos(at)</m> or <m>k \sin(at)</m></cell>
      <cell><m>C \cos(at) + D\sin(at)</m></cell>
    </row>
    <row>
      <cell><m>kt^n e^{at}</m></cell>
      <cell><m>e^{at}\left(C_n t^n + C_{n-1}t^{n-1} + \dots +
        C_1 t + C_0\right)</m></cell>
    </row>
    <row>
      <cell><m>k t^n \cos(at)</m> or <m>k t^n \sin(at)</m></cell>
      <cell><m>\left(C_nt^n + \dots +C_0 \right)\cos(at) + \left(D_nt^n +
        \dots + D_0 \right)\sin(at)</m></cell>
    </row>
    <row>
      <cell><m>ke^{at} \cos(bt)</m> or <m>ke^{at} \sin(bt)</m></cell>
      <cell><m>e^{at}\left(C \cos(at) + D\sin(at)\right)</m></cell>
    </row>
    <row>
      <cell><m>k t^n e^{at }\cos(bt)</m> or <m>k t^n e^{at} \sin(bt)</m></cell>
      <cell><m>\left(C_nt^n + \dots +C_0 \right)e^{at}\cos(bt)
        + \left(D_nt^n + \dots + D_0 \right)e^{bt}\sin(bt)</m></cell>
    </row>
  </tabular>
  <p>
    With this chart, the process is simple.
    We find the right guess,
    put it into the DE, and try to work out the unknown coefficients.
    Let's see this in examples.
  </p>
  <example>
    <statement>
      <p>
        This example is from Roberts and Marion.
        <md>
          <mrow>y^{\prime \prime} - 3y^\prime + 2y \amp  = t \hspace{2cm} y(0) = \frac{3}{4} \hspace{1cm} y^\prime(0) = \frac{3}{2}</mrow>
          <mrow>L \amp  = \frac{d^2}{dt^2} + 3 \frac{d}{dt} + 2</mrow>
          <mrow>\amp  \text{ Solve the Homogeneous Case: }</mrow>
          <mrow>Ly \amp  = 0 \implies r^2 - 3r + 2 = 0</mrow>
          <mrow>(r-2)(r-1) \amp  = 0 \implies r = 1,2</mrow>
          <mrow>y_h \amp  = A e^{2t} + B e^t</mrow>
          <mrow>\amp  \text{ Our Guess for Undetermined Coefficients: }</mrow>
          <mrow>y_p \amp  = Ct + D</mrow>
          <mrow>y_p^\prime \amp  = C</mrow>
          <mrow>y_p^{\prime \prime} \amp  = 0</mrow>
          <mrow>\amp  \text{ Solve for the Coefficients: }</mrow>
          <mrow>L y_p \amp  = 0 - 3C + 2(Ct + D) = t</mrow>
          <mrow>2C \amp  = 1 \implies C = \frac{1}{2}</mrow>
          <mrow>-3C + 2D \amp  = 0</mrow>
          <mrow>-3 \frac{1}{2} + 2 D \amp  = 0 \implies D =\frac{3}{4}</mrow>
          <mrow>y_p \amp  = \frac{t}{2} + \frac{3}{4}</mrow>
          <mrow>y \amp  = \frac{t}{2} + \frac{3}{4} + A e^{2t} + B e^t</mrow>
          <mrow>\amp  \text{ Use the Initial Values: }</mrow>
          <mrow>y(0) \amp  = \frac{3}{4} \hspace{1cm} y^\prime(0) = \frac{3}{2}</mrow>
          <mrow>y^\prime \amp  = 2Ae^{2t} + Be^t + \frac{1}{2}</mrow>
          <mrow>y(0) \amp  = A + B + \frac{3}{4} = \frac{3}{4} \implies A = -B</mrow>
          <mrow>y^\prime(0) \amp  = 2A + B + \frac{1}{2} = \frac{3}{2}</mrow>
          <mrow>2A + B \amp  = 1</mrow>
          <mrow>2A - B \amp  = 1 \implies A = 1 \implies B = -1</mrow>
          <mrow>y \amp  = \frac{t}{2} + \frac{3}{4} + e^{2t} - e^t</mrow>
        </md>
      </p>
    </statement>
  </example>
  <example>
    <statement>
      <p>
        This example lacks initial values.
        I've skipped over some of the algebra for the sake of brevity.
        <md>
          <mrow>y^{\prime \prime} + 8 y^\prime + 3y \amp  = e^{-2t} \cos 2t</mrow>
          <mrow>L \amp  = \frac{d^2}{dt^2} + 8 \frac{d}{dt} + 3</mrow>
          <mrow>\amp  \text{ Solve the Homogeneous Case: }</mrow>
          <mrow>Ly \amp  = 0 \implies r^2 + 8r + 3 = 0</mrow>
          <mrow>r \amp  = -4 \pm \sqrt{13}</mrow>
          <mrow>y_h \amp  = Ae^{(-4+\sqrt{13})t} + B e^{(-4-\sqrt{13})t}</mrow>
          <mrow>\amp  \text{ Our Guess for Undetermined Coefficients: }</mrow>
          <mrow>y_p \amp  = e^{-2t} (C \cos 2t + D \sin 2t)</mrow>
          <mrow>y^\prime \amp  = e^{-2t} ( (-2C + 2D) \cos 2t + (-2D -2C)\sin 2t)</mrow>
          <mrow>y^{\prime\prime} \amp  = e^{-2t} ( (-8D) \cos 2t + (8C)\sin 2t)</mrow>
          <mrow>\amp  \text{ Solve for the Coefficients: }</mrow>
          <mrow>L y_p \amp  = e^{-2t} ((8D-13C) \cos 2t + (-8C -13D) \sin 2t) = e^{-2t} \cos 2t</mrow>
          <mrow>8D - 13 C \amp  = 1</mrow>
          <mrow>-8C - 13 D \amp  = 0</mrow>
          <mrow>D \amp  = \frac{-8C}{13}</mrow>
          <mrow>C \amp  = \frac{-13}{233} \implies D = \frac{8}{233}</mrow>
          <mrow>y_p \amp  = e^{-2t} \left( \frac{-13}{233} \cos 2t + \frac{8}{233} \sin 2t \right)</mrow>
          <mrow>y \amp  = Ae^{(-4+\sqrt{13})t} + B e^{(-4-\sqrt{13})t} + e^{-2t} \left( \frac{-13}{233} \cos 2t + \frac{8}{233} \sin 2t \right)</mrow>
        </md>
      </p>
      <p>
        It's useful to go back to our harmonic system interpretation to understand these solutions.
        There are no oscillations in the homogeneous case here:
        sufficient friction gives exponential decay.
        However, there is oscillating forcing,
        though the forcing is also undering going exponential decay.
        This forcing is enough to add sinusoidal behaviour to the full solutions,
        but the decaying forcing terms means that the sinusoidal term will also decay over time.
        The amplitude of this combination of waves is given by the pythagorean combination:
        <m>\frac{\sqrt{13^2 + 8^2}}{233} = \frac{1}{\sqrt{233}}</m>.
      </p>
    </statement>
  </example>
  <example>
    <statement>
      <p>
        In this example,
        the forcing term is similar to one of the homogeneous solutions,
        so you will notice that we have multiplied by <m>t</m> in our guess for the particular solution.
        Again, I've skipped more of the algebra in this example,
        particularly omitting the long derivatives and calculation of <m>Ly_p</m>.
        <md>
          <mrow>y^{\prime \prime} + 2y^\prime + 2y \amp  = f(t) = 4e^{-t} \sin t</mrow>
          <mrow>\amp  \text{ Solve the Homogeneous Case: }</mrow>
          <mrow>r^2 + 2r + 2 \amp  = 0 \implies r = -1 \pm \imath</mrow>
          <mrow>y_h \amp  = e^{-t} (A \sin t + B \cos t)</mrow>
          <mrow>\amp  \text{ Our Guess for Undetermined Coefficients: }</mrow>
          <mrow>y_p \amp  = te^{-t} (C \sin t + D \cos t )</mrow>
          <mrow>y^{\prime} \amp  = e^{-t} (C \sin t + D \cos t) + te^{-t}((-C-D)\sin t + (-D+C)\cos t)</mrow>
          <mrow>y^{\prime\prime} \amp  = e^{-t} ((-2C-2D) \sin t + (-2D+2C) \cos t) + te^{-t}((2D)\sin t + (-2C)\cos t)</mrow>
          <mrow>\amp  \text{ Solve for the Coefficients: }</mrow>
          <mrow>L y_p \amp  = e^{-t} ((-2D) \sin t + (2C) \cos t) = 4e^{-t} \sin t</mrow>
          <mrow>-2D \amp  = 4 \implies D = -2</mrow>
          <mrow>2C \amp  = 0 \implies C = 0</mrow>
          <mrow>y_p \amp  = -2te^{-t} \cos t</mrow>
          <mrow>y \amp  = -2te^{-t} \cos t + e^{-t} (A \sin t + B \cos t)</mrow>
        </md>
      </p>
      <p>
        In this result, we still have exponential decay,
        since the exponential is asymptotically dominant in the <m>te^{-t}</m> term.
        However, the trajectory and behaviour of the decay differs,
        particular for small <m>t</m>,
        from the homogeneous solutions.
      </p>
    </statement>
  </example>
</section>