<section xml:id="variation-parameters">
  <title>Variation of Parameters</title>
  <introduction>
    <p>
      Undetermined coefficients is an effective and efficient
      (relatively speaking!)
      way to solve for a particular non-homogeneous solution of a SOLCCDE. It's restriction is its scope:
      it only works for specific forcing terms.
      Variation of parameters is a much more general method of finding particular solutions.
      It's weakness is the reliance on difficult integrals <mdash/> often we'll have to leave the solutions in a form which involves unfinished integrals.
      In the examples,
      we'll often stick to forcing terms which could have used undetermined coefficients,
      just to make the integrals reasonable.
    </p>
  </introduction>
  <subsection xml:id="wronskians">
    <title>Wronskians</title>
    <definition>
      <statement>
        <p>
          Let <m>f_1, f_2, \ldots f_n \in C^{n-1}(\RR)</m>.
          The <term>Wronskian</term> of this set of functions is defined to be the determinant of a matrix involving the <m>f_i</m> and their derivatives.
          <me>
            W(f_1, f_2, \ldots, f_n) : = \left| \begin{matrix} f_1 \amp  \ldots \amp  f_n \\ f^\prime_1 \amp  \ldots \amp  f^\prime_n \\ f^{\prime\prime}_1 \amp  \ldots \amp  f^{\prime\prime}_n \\ \ldots \amp  \ldots \amp  \ldots \\ f^{(n-1)}_1 \amp  \ldots \amp  f^{(n-1)}_n \end{matrix} \right|
          </me>
        </p>
      </statement>
    </definition>
    <p>
      The Wronskian of a set of functions has a number of different uses.
      Its first use is checking for linear independence.
      The set of functions linearly independent if and only if the Wronskian is never zero.
      Most of the time, this is easy to satisfy.
      In addition, if we have linearly independent functions,
      we know the Wronskian is never zero and we can divide by if with impunity.
    </p>
    <p>
      For variation of parameters, we only need to the Wronskain of two functions.
      The definition here is relatively simple.
      <me>
        W(f_1,f_2) = \left| \begin{matrix} f_1 \amp  f_2 \\ f_1^\prime \amp f_2^\prime \end{matrix} \right| = f_1 f_2^\prime - f_2 f_1^\prime
      </me>
    </p>
  </subsection>
  <subsection xml:id="technique-vop">
    <title>The Technique of Variations of Parameters</title>
    <p>
      Let <m>L</m> be the second order operator
      <me>
        L = \frac{d^2}{dt^2} +P \frac{d}{dt} + Q
      </me>.
    </p>
    <p>
      Let <m>y_1</m> and <m>y_2</m> be solutions to the homogeneous equation <m>Ly=0</m>.
      The general solution to the homogeneous equation is <m>Ay_1 + By_2</m>.
      As with the first-order case,
      variation of parameters replaces the constants <m>A</m> and <m>B</m> with functions.
      That is, we look for a solution which has the form (where <m>u_1(t)</m> and <m>u_2(t)</m> are unknown functions)
      <me>
        y_p = u_1 y_1 + u_2 y_2
      </me>.
    </p>
    <p>
      Then we put this <m>y_p</m> into the differential equation.
      A long and tedious calculation ensues.
      <md>
        <mrow>Ly_p \amp  = u_1^{\prime \prime} y_1 + 2 u_1^\prime y_1^\prime + u_1 y_1^{\prime \prime} + u_2^{\prime \prime} y_2 + 2 u_2^\prime y_2^\prime + u_2 y_2^{\prime \prime} + P \left( u_1^\prime y_1 + u_1 y_1^\prime + u_2^\prime y_2 + u_2 y_2^\prime \right)</mrow>
        <mrow>\amp  \hspace{2cm}+ Q \left( u_1 y_1 + u_2 y_2 \right) = f</mrow>
        <mrow>\amp  = u_1 \left( y_1^{\prime \prime} + Py_1^\prime + Q y_1 \right) + u_2 \left( y_2^{\prime \prime} + Py_2^\prime + Q y_2 \right) + (y_1 u_1^{\prime \prime} + u_1^\prime y_1^\prime) + (y_2 u_2^{\prime \prime} + u_2^\prime y_2^\prime)</mrow>
        <mrow>\amp  \hspace{2cm} + P \left( y_1 u_1^\prime + y_2 u_2^\prime \right) + y_1^\prime u_1^\prime + y_2^\prime u_2^\prime = f</mrow>
        <mrow>\amp  = u_1 (L y_1) + u_2 (L y_2) + \frac{d}{dt} \left( y_1 u_1^\prime \right) + \frac{d}{dt} \left( y_2 u_2^\prime \right) + P \left( y_1 u_1^\prime + y_2 u_2^\prime \right) + \left( y_1^\prime u_1^\prime + y_2^\prime u_2^\prime \right) = f</mrow>
        <mrow>\amp  = 0 + 0 + \frac{d}{dt} \left(y_1 u_1^\prime + y_2 u_2^\prime \right) + P \left( y_1 u_1^\prime + y_2 u_2^\prime \right) + \left( y_1^\prime u_1^\prime + y_2^\prime u_2^\prime \right) = f</mrow>
      </md>
    </p>
    <p>
      So far, this doesn't look particularly useful.
      Part of the problem is that we've given ourselves too much freedom.
      Choosing two entirely unknown functions is not limiting enough.
      The advantage of this situation is that we can impose a reasonable restriction while still allowing for general solutions.
      We impose the restriction <m>y_1 u_1^\prime + y_2 u_2^\prime = 0</m>.
      (Why this restriction?
      Because it works, and somewhere in matheamtical history,
      some clever mathematician figured out that it works.)
      This restriction removes two terms from the previous equation and leaves us with a simple equation.
      <me>
        \left( y_1^\prime u_1^\prime + y_2^\prime u_2^\prime \right) = f
      </me>
    </p>
    <p>
      If we remember the restriction,
      we now have a system of two equations.
      <md>
        <mrow>y_1 u_1^\prime + y_2 u_2^\prime \amp  = 0</mrow>
        <mrow>y_1^\prime u_1^\prime + y_2^\prime u_2^\prime \amp  = f</mrow>
      </md>
    </p>
    <p>
      We can express this system in matrix terminology.
      <me>
        \begin{pmatrix}0\\f\end{pmatrix} = \left( \begin{matrix} y_1 \amp  y_2 \\ y_1^\prime \amp  y_2^\prime \end{matrix} \right) \begin{pmatrix}u_1^\prime\\u_2^\prime\end{pmatrix}
      </me>
    </p>
    <p>
      Linear algebra then solves the system.
      Conveniently,
      the determinant of the system is the Wronskian <m>W(y_1,y_2)</m>,
      which we will simply write <m>W</m> for the remainder of this derivation.
      <md>
        <mrow>u_1^\prime \amp  = \frac{-y_2 f}{W}</mrow>
        <mrow>u_2^\prime \amp  = \frac{y_1 f}{W}</mrow>
      </md>
    </p>
    <p>
      The solution gives us the derivatives of <m>u_1</m> and <m>u_2</m>,
      so we can integrate.
      <md>
        <mrow>u_1 \amp  = - \int \frac{y_2 f}{W} dt</mrow>
        <mrow>u_2 \amp  = \int \frac{y_1 f}{W} dt</mrow>
      </md>
    </p>
    <p>
      We insert these <m>u_i</m> in the original expression.
      <me>
        y_p = \left( -\int \frac{y_2 f}{W} dt \right) y_1 + \left( \int \frac{y_1 f}{W} dt \right) y_2
      </me>
    </p>
    <p>
      Therefore, the general solution to the original equation <m>Ly = f</m> is
      <me>
        y_p = \left( -\int \frac{y_2 f}{W} dx \right) y_1 + \left( \int \frac{y_1 f}{W} dt \right) y_2 + Ay_1 + By_2
      </me>.
    </p>
    <p>
      Note that this general form implies, conveniently,
      that we don't have to worry about constants of integration in either of the two integrals.
      If we had a constant of integration,
      it would lead to a multiple of one of the homogeneous solutions.
      Those multiples are already accounted for in the general homogeneous solution.
    </p>
    <example>
      <statement>
        <p>
          This example is from Roberts and Marion.
          <md>
            <mrow>y^{\prime\prime} - 2y^{\prime} + 2y \amp  = 2e^t</mrow>
            <mrow>r^2 -2r +2 \amp  = 0</mrow>
            <mrow>r \amp  = 1 \pm \imath</mrow>
            <mrow>y_1 \amp  = e^t \cos t</mrow>
            <mrow>y_2 \amp  = e^t \sin t</mrow>
            <mrow>y_1^\prime \amp  = e^t \cos t - e^t \sin t</mrow>
            <mrow>y_2^\prime \amp  = e^t \sin t + e^t \cos t</mrow>
            <mrow>W \amp  = e^t \cos t (e^t \sin t + e^t \cos t) - e^t \sin t (e^t \cos t - e^t \sin t)</mrow>
            <mrow>\amp  = e^{2t} (\cos t \sin t + \cos^2 t - \sin t \cos t + \sin^2 t) = e^{2t}</mrow>
            <mrow>u_1 \amp  = \int \frac{-y_2 f}{W} dt = -\int \frac{ e^t \sin t 2e^t}{e^{2t}}dt</mrow>
            <mrow>\amp  = -2 \int \sin t dt = 2 \cos t</mrow>
            <mrow>u_2 \amp  = \int \frac{y_1 f}{W} dt = \int \frac{ e^t \cos t 2e^t}{e^{2t}}dt</mrow>
            <mrow>\amp  = 2 \int \cos t dt = 2 \sin t</mrow>
            <mrow>y_p \amp  = 2\cos t e^t \cos t + 2 \sin t e^t \sin t = 2e^t</mrow>
            <mrow>y \amp  = 2e^t + Ae^t \cos t + B e^t \sin t</mrow>
          </md>
        </p>
      </statement>
    </example>
    <example>
      <statement>
        <md>
          <mrow>y^{\prime\prime} - 4y^{\prime} + 4y \amp  = (t+1)e^{2t}</mrow>
          <mrow>r^2 -4r +4 \amp  = 0</mrow>
          <mrow>r \amp  = 2</mrow>
          <mrow>y_1 \amp  = e^{2t}</mrow>
          <mrow>y_2 \amp  = te^{2t}</mrow>
          <mrow>y_1^\prime \amp  = 2e^{2t}</mrow>
          <mrow>y_2^\prime \amp  = 2te^{2t} + e^{2t}</mrow>
          <mrow>W \amp  = e^{2t} (e^{2t} + 2te^{2t}) - te^{2t} 2e^{2t} = e^{4t}</mrow>
          <mrow>u_1 \amp  = \int \frac{-y_2 f}{W} dt = -\int
          \frac{te^{2t}(t+1)e^{2t}}{e^{4t}} dt</mrow>
          <mrow>\amp  = - \int t^2 + t = \frac{-t^3}{3} - \frac{t^2}{2}</mrow>
          <mrow>u_2 \amp  = \int \frac{y_1 f}{W} dt = \int \frac{ e^{2t}
          (t+1)e^{2t}}{e^{4t}} dt</mrow>
          <mrow>\amp  = \int t+1 dt = \frac{t^2}{2} + t</mrow>
          <mrow>y_p \amp  = \left( \frac{-t^3}{3} - \frac{t^2}{2} \right) e^{2t} +
          \left( \frac{t^2}{2} + t \right) te^{2t}</mrow>
          <mrow>\amp  = \frac{t^3 e^{2t}}{6} + \frac{t^2e^2t}{2}</mrow>
          <mrow>y \amp  = \frac{t^3 e^{2t}}{6} + \frac{t^2e^2t}{2} + Ae^{2t} +
          Bte^{2t}</mrow>
        </md>
      </statement>
    </example>
    <example>
      <statement>
        <p>
          This is (finally) an example that couldn't have used undetermined coefficients.
          <md>
            <mrow>y^{\prime\prime} + 9y \amp  = \csc 3t</mrow>
            <mrow>r^2 + 9 \amp  = 0</mrow>
            <mrow>r \amp  = \pm 3\imath</mrow>
            <mrow>y_1 \amp  = \cos 3t</mrow>
            <mrow>y_2 \amp  = \sin 3t</mrow>
            <mrow>y_1^\prime \amp  = -3 \sin 3t</mrow>
            <mrow>y_2^\prime \amp  = 3 \cos 3t</mrow>
            <mrow>W \amp  = 3\cos^2 3t + 3 \sin^2 3t = 3</mrow>
            <mrow>u_1 \amp  = \int \frac{-y_2 f}{W} dt = -\int \frac{\sin 3t \csc 3t}{3} dt = \frac{-1}{3} \int dt = \frac{-t}{3}</mrow>
            <mrow>u_2 \amp  = \int \frac{y_1 f}{W} dt = \int \frac{\cos3t \csc 3t}{3} dt = \frac{1}{3} \int \cot 3t = \frac{1}{9} \ln |\sin 3t|</mrow>
            <mrow>y_p \amp  = \frac{-t}{3} \cos 3t + \frac{\sin 3t \ln |\sin 3t|}{9}</mrow>
            <mrow>y \amp  = \frac{-t}{3} \cos 3t + \frac{\sin 3t \ln |\sin 3t|}{9} + A \cos 3t + B \sin 3t</mrow>
          </md>
        </p>
        <p>
          One of the reasons that undetermined coefficients wouldn't have worked is that the form of the particular solution,
          <m>\ln |\sin 3t|</m>, is not a function likely to be guessed.
        </p>
      </statement>
    </example>
    <example>
      <statement>
        <p>
          In this example,
          the resulting integrals are not expressable by elementary functions.
          In these cases, we just leave the integrals in the final solution.
          We just have to live with these unexpressible function (or, I suppose,
          come up with new names for them.)
          <md>
            <mrow>y^{\prime\prime} - y \amp  = \frac{1}{t}</mrow>
            <mrow>r^2 - 1 \amp  = 0</mrow>
            <mrow>r \amp  = \pm 1</mrow>
            <mrow>y_1 \amp  = e^t</mrow>
            <mrow>y_2 \amp  = e^{-t}</mrow>
            <mrow>y_1^\prime \amp  = e^t</mrow>
            <mrow>y_2^\prime \amp  = - e^{-t}</mrow>
            <mrow>W \amp  = -1 -1 = -2</mrow>
            <mrow>u_1 \amp  = \int \frac{-y_2 f}{W} dt = -\int \frac{ e^{-t} \frac{1}{t}}{-2} = \frac{1}{2} \int \frac{e^{-t}}{t} dt</mrow>
            <mrow>u_2 \amp  = \int \frac{y_1 f}{W} dt = \int \frac{ e^t \frac{1}{t}}{-2} = \frac{-1}{2} \int \frac{e^t}{t} dt</mrow>
            <mrow>y_p \amp  = \frac{e^t}{2} \int \frac{e^{-t}}{t} dt - \frac{e^{-t}}{2} \int \frac{e^t}{t} dt</mrow>
            <mrow>y \amp  = \frac{e^t}{2} \int \frac{e^{-t}}{t} dt - \frac{e^{-t}}{2} \int \frac{e^t}{t} dt + Ae^t + Be^{-t}</mrow>
          </md>
        </p>
      </statement>
    </example>
  </subsection>
</section>